src/lang/Memory.v
@@ -7,15 +7,152 @@ Require Import paco.
 Require Import Axioms.
 Require Import Basic.
 Require Import DataStructure.
+Require Import DenseOrder.
 Require Import Event.
 Require Import Time.
 
 Set Implicit Arguments.
 
 
+Module Promises.
+  Definition t := Loc.t -> DOSet.t.
+
+  Definition mem loc ts (promises:t) := DOSet.mem ts (promises loc).
+
+  Lemma ext lhs rhs
+        (EXT: forall loc ts, mem loc ts lhs = mem loc ts rhs):
+    lhs = rhs.
+  Proof.
+    extensionality loc.
+    apply DOSet.eq_leibniz. ii.
+    specialize (EXT loc a). unfold mem in *. econs; i.
+    - apply DOSet.mem_spec. erewrite <- EXT.
+      apply DOSet.mem_spec. auto.
+    - apply DOSet.mem_spec. erewrite EXT.
+      apply DOSet.mem_spec. auto.
+  Qed.
+
+  Definition bot: t := fun _ => DOSet.empty.
+
+  Lemma bot_spec loc ts: mem loc ts bot = false.
+  Proof.
+    unfold mem, bot. apply DOSet.Facts.empty_b.
+  Qed.
+
+  Definition le (lhs rhs:t): Prop :=
+    forall loc ts, mem loc ts lhs -> mem loc ts rhs.
+
+  Definition join (lhs rhs:t): t :=
+    fun loc => DOSet.union (lhs loc) (rhs loc).
+
+  Lemma join_comm lhs rhs: join lhs rhs = join rhs lhs.
+  Proof.
+    unfold join. extensionality loc.
+    apply DOSet.eq_leibniz. ii.
+    rewrite ? DOSet.union_spec. econs; i; des; auto.
+  Qed.
+
+  Lemma join_assoc a b c: join (join a b) c = join a (join b c).
+  Proof.
+    unfold join. extensionality loc.
+    apply DOSet.eq_leibniz. ii.
+    rewrite ? DOSet.union_spec. econs; i; des; auto.
+  Qed.
+
+  Lemma join_l lhs rhs: le lhs (join lhs rhs).
+  Proof.
+    unfold join. ii. unfold mem in *.
+    rewrite DOSet.Facts.union_b, H. auto.
+  Qed.
+
+  Lemma join_r lhs rhs: le rhs (join lhs rhs).
+  Proof. rewrite join_comm. apply join_l. Qed.
+
+  Lemma join_spec lhs rhs o
+        (LHS: le lhs o)
+        (RHS: le rhs o):
+    le (join lhs rhs) o.
+  Proof.
+    unfold join. ii.
+    unfold mem in *. rewrite DOSet.Facts.union_b in *.
+    apply Bool.orb_true_iff in H. des; eauto.
+  Qed.  
+
+  Definition set (loc:Loc.t) (ts:Time.t) (promises:t) :=
+    LocFun.add loc (DOSet.add ts (promises loc)) promises.
+
+  Lemma set_o loc1 ts1 loc2 ts2 promises:
+    mem loc1 ts1 (set loc2 ts2 promises) =
+    if andb (if Loc.eq_dec loc1 loc2 then true else false) (if Time.eq_dec ts1 ts2 then true else false)
+    then true
+    else mem loc1 ts1 promises.
+  Proof.
+    unfold mem, set, LocFun.add, LocFun.find.
+    destruct (Loc.eq_dec loc1 loc2); subst; ss.
+    destruct (Time.eq_dec ts1 ts2); subst; ss.
+    - rewrite DOSet.Facts.add_b.
+      unfold DOSet.Facts.eqb. destruct (Time.eq_dec ts2 ts2); auto.
+    - rewrite DOSet.Facts.add_b.
+      unfold DOSet.Facts.eqb. destruct (Time.eq_dec ts2 ts1); ss.
+      congruence.
+  Qed.
+
+  Lemma set_inv loc1 ts1 loc2 ts2 promises
+        (MEM: mem loc1 ts1 (set loc2 ts2 promises)):
+    (loc1 = loc2 /\ ts1 = ts2) \/ mem loc1 ts1 promises.
+  Proof.
+    rewrite set_o in MEM.
+    destruct (Loc.eq_dec loc1 loc2); ss; auto.
+    destruct (Time.eq_dec ts1 ts2); ss; auto.
+  Qed.
+
+  Definition unset (loc:Loc.t) (ts:Time.t) (promises:t) :=
+    LocFun.add loc (DOSet.remove ts (promises loc)) promises.
+
+  Lemma unset_o loc1 ts1 loc2 ts2 promises:
+    mem loc1 ts1 (unset loc2 ts2 promises) =
+    if andb (if Loc.eq_dec loc1 loc2 then true else false) (if Time.eq_dec ts1 ts2 then true else false)
+    then false
+    else mem loc1 ts1 promises.
+  Proof.
+    unfold mem, unset, LocFun.add, LocFun.find.
+    destruct (Loc.eq_dec loc1 loc2); subst; ss.
+    destruct (Time.eq_dec ts1 ts2); subst; ss.
+    - rewrite DOSet.Facts.remove_b.
+      unfold DOSet.Facts.eqb. destruct (Time.eq_dec ts2 ts2); [|congruence].
+      apply Bool.andb_false_iff. auto.
+    - rewrite DOSet.Facts.remove_b.
+      unfold DOSet.Facts.eqb. destruct (Time.eq_dec ts2 ts1); ss; [congruence|].
+      apply Bool.andb_true_r.
+  Qed.
+
+  Lemma unset_inv loc1 ts1 loc2 ts2 promises
+        (MEM: mem loc1 ts1 (unset loc2 ts2 promises)):
+    ~ (loc1 = loc2 /\ ts1 = ts2) /\ mem loc1 ts1 promises.
+  Proof.
+    rewrite unset_o in MEM.
+    destruct (Loc.eq_dec loc1 loc2), (Time.eq_dec ts1 ts2); ss; splits; auto.
+    - contradict n. des. auto.
+    - contradict n. des. auto.
+    - contradict n. des. auto.
+  Qed.
+
+  Inductive disjoint (lhs rhs:t): Prop :=
+  | disjoint_intro
+      (DISJOINT: forall loc ts
+                   (LHS: mem loc ts lhs)
+                   (RHS: mem loc ts rhs),
+          False).
+
+  Global Program Instance disjoint_Symmetric: Symmetric disjoint.
+  Next Obligation.
+    econs. ii. eapply H; eauto.
+  Qed.
+End Promises.
+
 Module TimeMap <: JoinableType.
-  Definition t := LocFun.t Time.t.
-  Definition elt: t := LocFun.init Time.elt.
+  Definition t := Loc.t -> Time.t.
+  Definition elt: t := fun _ => Time.elt.
 
   Definition eq := @eq t.
 
@@ -26,15 +163,13 @@ Module TimeMap <: JoinableType.
   Next Obligation. ii. reflexivity. Qed.
   Next Obligation. ii. etrans; eauto. Qed.
 
-  Definition get (loc:Loc.t) (c:t) := LocFun.find loc c.
+  Definition get (loc:Loc.t) (c:t) := c loc.
 
   Definition join (lhs rhs:t): t :=
     fun loc => Time.join (lhs loc) (rhs loc).
 
   Lemma join_comm lhs rhs: join lhs rhs = join rhs lhs.
-  Proof.
-    unfold join. extensionality loc. apply Time.join_comm.
-  Qed.
+  Proof. unfold join. extensionality loc. apply Time.join_comm. Qed.
 
   Lemma join_assoc a b c: join (join a b) c = join a (join b c).
   Proof.
@@ -43,22 +178,16 @@ Module TimeMap <: JoinableType.
   Qed.
 
   Lemma join_l lhs rhs: le lhs (join lhs rhs).
-  Proof.
-    ii. apply Time.join_l.
-  Qed.
+  Proof. ii. apply Time.join_l. Qed.
 
   Lemma join_r lhs rhs: le rhs (join lhs rhs).
-  Proof.
-    ii. apply Time.join_r.
-  Qed.
+  Proof. ii. apply Time.join_r. Qed.
 
   Lemma join_spec lhs rhs o
         (LHS: le lhs o)
         (RHS: le rhs o):
     le (join lhs rhs) o.
-  Proof.
-    unfold join. ii. apply Time.join_spec; auto.
-  Qed.
+  Proof. unfold join. ii. apply Time.join_spec; auto. Qed.
 
   Definition incr loc ts c :=
     LocFun.add loc (Time.join (c loc) ts) c.
@@ -110,6 +239,12 @@ Module Capability <: JoinableType.
   }.
   Definition t := t_.
 
+  Inductive wf (capability:t): Prop :=
+  | wf_intro
+      (UR_RW: TimeMap.le capability.(ur) capability.(rw))
+      (RW_SC: TimeMap.le capability.(rw) capability.(sc))
+  .
+
   Definition elt: t := mk TimeMap.elt TimeMap.elt TimeMap.elt.
 
   Definition eq := @eq t.
@@ -136,9 +271,7 @@ Module Capability <: JoinableType.
        (TimeMap.join lhs.(sc) rhs.(sc)).
 
   Lemma join_comm lhs rhs: join lhs rhs = join rhs lhs.
-  Proof.
-    unfold join. f_equal; apply TimeMap.join_comm.
-  Qed.
+  Proof. unfold join. f_equal; apply TimeMap.join_comm. Qed.
 
   Lemma join_assoc a b c: join (join a b) c = join a (join b c).
   Proof.
@@ -149,14 +282,10 @@ Module Capability <: JoinableType.
   Qed.
 
   Lemma join_l lhs rhs: le lhs (join lhs rhs).
-  Proof.
-    econs; apply TimeMap.join_l.
-  Qed.
+  Proof. econs; apply TimeMap.join_l. Qed.
 
   Lemma join_r lhs rhs: le rhs (join lhs rhs).
-  Proof.
-    econs; apply TimeMap.join_r.
-  Qed.
+  Proof. econs; apply TimeMap.join_r. Qed.
 
   Lemma join_spec lhs rhs o
         (LHS: le lhs o)
@@ -167,10 +296,60 @@ Module Capability <: JoinableType.
     econs; apply TimeMap.join_spec; eauto.
   Qed.
 
+  Lemma join_wf
+        lhs rhs
+        (LHS: wf lhs)
+        (RHS: wf rhs):
+    wf (join lhs rhs).
+  Proof.
+    econs.
+    - apply TimeMap.join_spec.
+      + etrans; [apply LHS|]. apply TimeMap.join_l.
+      + etrans; [apply RHS|]. apply TimeMap.join_r.
+    - apply TimeMap.join_spec.
+      + etrans; [apply LHS|]. apply TimeMap.join_l.
+      + etrans; [apply RHS|]. apply TimeMap.join_r.
+  Qed.
+
+  Definition join_if (cond:bool) (a b:t): t :=
+    if cond then join a b else b.
+
+  Lemma join_if_wf
+        cond lhs rhs
+        (LHS: wf lhs)
+        (RHS: wf rhs):
+    wf (join_if cond lhs rhs).
+  Proof.
+    destruct cond; ss. apply join_wf; auto.
+  Qed.
+
+  Lemma join_if_spec
+        (cond:bool) a b c
+        (A: cond -> le a c)
+        (B: le b c):
+    le (join_if cond a b) c.
+  Proof. destruct cond; auto. apply join_spec; auto. Qed.
+
+  Lemma join_if_le
+        (cond:bool) a b c
+        (A: cond -> le c a)
+        (B: ~cond -> le c b):
+    le c (if cond then a else b).
+  Proof. destruct cond; auto. Qed.
+
   Definition incr_ur loc ts s :=
     mk (TimeMap.incr loc ts s.(ur))
        (TimeMap.incr loc ts s.(rw))
        (TimeMap.incr loc ts s.(sc)).
+
+  Lemma incr_ur_wf loc ts s
+        (WF: wf s):
+    wf (incr_ur loc ts s).
+  Proof.
+    econs; s.
+    - apply TimeMap.incr_mon. apply WF.
+    - apply TimeMap.incr_mon. apply WF.
+  Qed.
 
   Lemma incr_ur_le
         loc ts s:
@@ -227,6 +406,15 @@ Module Capability <: JoinableType.
        (TimeMap.incr loc ts s.(rw))
        (TimeMap.incr loc ts s.(sc)).
 
+  Lemma incr_rw_wf loc ts s
+        (WF: wf s):
+    wf (incr_rw loc ts s).
+  Proof.
+    econs; s.
+    - etrans; [|apply TimeMap.incr_le]. apply WF.
+    - apply TimeMap.incr_mon. apply WF.
+  Qed.
+
   Lemma incr_rw_le
         loc ts s:
     le s (incr_rw loc ts s).
@@ -271,27 +459,6 @@ Module Capability <: JoinableType.
     - apply TimeMap.incr_ts.
     - apply TimeMap.incr_ts.
   Qed.
-
-  Definition join_if (cond:bool) (a b:t): t :=
-    if cond then join a b else b.
-
-  Lemma join_if_spec
-        (cond:bool) a b c
-        (A: cond -> le a c)
-        (B: le b c):
-    le (join_if cond a b) c.
-  Proof.
-    destruct cond; auto. apply join_spec; auto.
-  Qed.
-
-  Lemma join_if_le
-        (cond:bool) a b c
-        (A: cond -> le c a)
-        (B: ~cond -> le c b):
-    le c (if cond then a else b).
-  Proof.
-    destruct cond; auto.
-  Qed.
 End Capability.
 
 Module Message.
@@ -304,599 +471,157 @@ End Message.
 
 Module Cell.
   Module Raw.
-    Structure t := mk {
-      messages: Time.t -> option Message.t;
-      ownership: Time.t -> bool;
-    }.
-
-    Definition get (ts:Time.t) (cell:t): option Message.t := cell.(messages) ts.
-
-    Inductive belongs_to (cell:t) (ts to:Time.t): Prop :=
-    | belongs_to_instro
-        from msg
-        (TS: Interval.mem (from, to) ts)
-        (OWN: Interval.mem (from, to) <1= cell.(ownership))
-        (MSG: cell.(messages) to = Some msg)
-    .
+    Definition t := DOMap.t (DenseOrder.t * Message.t).
 
     Inductive wf (cell:t): Prop :=
     | wf_intro
-        (MSG: forall ts msg, cell.(messages) ts = Some msg -> cell.(ownership) ts)
-        (OWN: forall ts, cell.(ownership) ts -> exists to, belongs_to cell ts to)
-        (FINITE: exists tos, forall ts msg, cell.(messages) ts = Some msg -> List.In ts tos)
+        (VOLUME: forall from to msg
+                   (GET: DOMap.find to cell = Some (from, msg)),
+            Time.lt from to)
+        (DISJOINT: forall to1 to2 from1 from2 msg1 msg2
+                     (GET1: DOMap.find to1 cell = Some (from1, msg1))
+                     (GET2: DOMap.find to2 cell = Some (from2, msg2))
+                     (NEQ: to1 <> to2),
+            Interval.disjoint (from1, to1) (from2, to2))
     .
 
-    Lemma extensionality
-          (cell1 cell2:t)
-          (EQ: forall to, cell1.(messages) to = cell2.(messages) to /\ cell1.(ownership) to = cell2.(ownership) to):
-      cell1 = cell2.
-    Proof.
-      destruct cell1, cell2.
-      assert (messages0 = messages1); subst.
-      { apply TimeFun.extensionality. apply EQ. }
-      assert (ownership0 = ownership1); subst.
-      { apply TimeFun.extensionality. i. apply EQ. }
-      auto.
-    Qed.
+    Definition get (ts:Time.t) (cell:t): option Message.t :=
+      option_map snd (DOMap.find ts cell).
 
-    Lemma extensionality_inv lhs rhs (EQ: lhs = rhs):
-      <<MSG: forall to, lhs.(messages) to = rhs.(messages) to>> /\
-      <<OWN: forall to, lhs.(ownership) to = rhs.(ownership) to>>.
-    Proof. subst. auto. Qed.
+    Inductive le (lhs rhs:t): Prop :=
+    | le_intro
+        (LE: forall from to msg
+               (GET: DOMap.find to lhs = Some (from, msg)),
+            DOMap.find to rhs = Some (from, msg))
+    .
+
+    Global Program Instance le_PreOrder: PreOrder le.
+    Next Obligation.
+      econs. i. auto.
+    Qed.
+    Next Obligation.
+      econs. i. apply H0. apply H. auto.
+    Qed.
 
     Inductive disjoint (lhs rhs:t): Prop :=
     | disjoint_intro
-        (DISJOINT: forall ts, lhs.(ownership) ts -> rhs.(ownership) ts -> False)
+        (DISJOINT: forall to1 to2 from1 from2 msg1 msg2
+                     (GET1: DOMap.find to1 lhs = Some (from1, msg1))
+                     (GET2: DOMap.find to2 rhs = Some (from2, msg2)),
+            Interval.disjoint (from1, to1) (from2, to2))
     .
 
     Global Program Instance disjoint_Symmetric: Symmetric disjoint.
     Next Obligation.
-      inv H. econs. i. eapply DISJOINT; eauto.
+      inv H. econs. i. symmetry. eapply DISJOINT; eauto.
     Qed.
 
-    Lemma disjoint_messages
-          lhs rhs
-          ts lmsg rmsg
-          (LWF: wf lhs)
-          (RWF: wf rhs)
-          (DISJOINT: disjoint lhs rhs)
-          (LMSG: lhs.(messages) ts = Some lmsg)
-          (RMSG: rhs.(messages) ts = Some rmsg):
-      False.
-    Proof.
-      eapply DISJOINT.
-      - inv LWF. eapply MSG. eauto.
-      - inv RWF. eapply MSG. eauto.
-    Qed.
-
-    Definition join (lhs rhs:t): t :=
-      mk (fun t =>
-            match lhs.(messages) t, rhs.(messages) t with
-            | Some _, Some _ => Some Message.elt
-            | Some _, None => lhs.(messages) t
-            | None, _ => rhs.(messages) t
-            end)
-         (fun t => orb (lhs.(ownership) t) (rhs.(ownership) t)).
-
-    Lemma join_comm lhs rhs:
-      join lhs rhs = join rhs lhs.
-    Proof.
-      unfold join. apply extensionality. s. i. splits.
-      - destruct (messages lhs to), (messages rhs to); auto.
-      - apply Bool.orb_comm.
-    Qed.
-
-    Lemma join_assoc a b c:
-      join a (join b c) = join (join a b) c.
-    Proof.
-      unfold join. apply extensionality. s. i. splits.
-      - destruct (messages a to), (messages b to), (messages c to); auto.
-      - apply Bool.orb_assoc.
-    Qed.
-
-    Lemma join_disjoint a b c:
-      disjoint a (join b c) <-> disjoint a b /\ disjoint a c.
-    Proof.
-      unfold join. econs; intro X; inv X; ss.
-      - splits; econs; i.
-        + eapply DISJOINT; eauto. rewrite H0. auto.
-        + eapply DISJOINT; eauto. rewrite H0. rewrite Bool.orb_comm. auto.
-      - econs; s; i; des.
-        apply Bool.orb_true_iff in H2. des.
-        + eapply H; eauto.
-        + eapply H0; eauto.
-    Qed.
-
-    Lemma join_wf a b
-          (WFA: wf a)
-          (WFB: wf b):
-      wf (join a b).
-    Proof.
-      econs; s; i.
-      - destruct (messages a ts) eqn:A.
-        { inv WFA. rewrite MSG; eauto. }
-        destruct (messages b ts) eqn:B.
-        { inv WFB. rewrite MSG; eauto. apply Bool.orb_comm. }
-        inv H.
-      - apply Bool.orb_true_iff in H. des.
-        + inversion WFA. exploit OWN; eauto. i. des.
-          exists to. inv x. econs; s; eauto.
-          * i. apply Bool.orb_true_iff. left. eapply OWN0; eauto.
-          * rewrite MSG0.
-            instantiate (1 := match messages b to with
-                              | Some _ => Message.elt
-                              | None => msg
-                              end).
-            destruct (messages b to); auto.
-        + inversion WFB. exploit OWN; eauto. i. des.
-          exists to. inv x. econs; s; eauto.
-          * i. apply Bool.orb_true_iff. right. eapply OWN0; eauto.
-          * rewrite MSG0.
-            instantiate (1 := match messages a to with
-                              | Some _ => Message.elt
-                              | None => msg
-                              end).
-            destruct (messages a to); auto.
-      - inv WFA. inv WFB. des.
-        exists (tos0 ++ tos). i. apply List.in_app_iff.
-        destruct (messages a ts) eqn:A.
-        { left. eapply FINITE. eauto. }
-        destruct (messages b ts) eqn:B.
-        { right. eapply FINITE0. eauto. }
-        inv H.
-    Qed.
-
-    Definition bot: t :=
-      mk (fun _ => None) (fun _ => false).
+    Definition bot: t := DOMap.empty _.
 
     Lemma bot_wf: wf bot.
     Proof.
-      unfold bot. econs; s; i.
-      - inv H.
-      - inv H.
-      - exists []. ii. inv H.
+      econs; i.
+      - rewrite DOMap.gempty in GET. inv GET.
+      - rewrite DOMap.gempty in GET1. inv GET1.
     Qed.
 
-    Lemma bot_disjoint cell: disjoint cell bot.
-    Proof. econs. i. inv H0. Qed.
+    Lemma bot_le cell: le bot cell.
+    Proof. econs. i. rewrite DOMap.gempty in GET. inv GET. Qed.
 
-    Lemma bot_join cell: join cell bot = cell.
-    Proof.
-      unfold join. apply extensionality. s. i. splits.
-      - destruct (messages cell to); auto.
-      - apply Bool.orb_false_r.
-    Qed.
-
-    Lemma bot_join_inv a b
-          (A: wf a)
-          (B: wf b)
-          (EQ: a = join a b)
-          (DISJOINT: disjoint a b):
-      b = bot.
-    Proof.
-      apply extensionality_inv in EQ. des.
-      apply extensionality. i.
-      specialize (MSG to). specialize (OWN to).
-      inv DISJOINT. specialize (DISJOINT0 to). ss.
-      destruct (ownership a to) eqn:OA, (ownership b to) eqn:OB,
-               (messages a to) eqn:MA, (messages b to) eqn:MB;
-        inv MSG; inv OWN; intuition.
-      - inv B. exploit MSG; eauto. congruence.
-      - inv A. exploit MSG; eauto. congruence.
-    Qed.
+    Lemma bot_disjoint cell: disjoint bot cell.
+    Proof. econs. i. rewrite DOMap.gempty in GET1. inv GET1. Qed.
 
     Definition singleton (from to:Time.t) (msg:Message.t): t :=
-      mk (fun ts => if Time.eq_dec ts to then Some msg else None)
-         (fun ts => if Interval.mem_dec (from, to) ts then true else false).
+      DOMap.singleton to (from, msg).
 
     Lemma singleton_wf
           from to msg
           (LT: Time.lt from to):
       wf (singleton from to msg).
     Proof.
-      unfold singleton. econs; s; i; timetac.
-      - exists to. econs; s; i; timetac.
-        + econs; eauto.
-        + inv PR. timetac.
-        + inv PR. timetac.
-      - exists [to]. i. timetac.
+      unfold singleton. econs; s; i.
+      - apply DOMap.singleton_find_inv in GET. des. inv GET0.
+        auto.
+      - apply DOMap.singleton_find_inv in GET1. des. inv GET0.
+        apply DOMap.singleton_find_inv in GET2. des. inv GET0.
+        congruence.
     Qed.
 
-    Inductive splits (lhs rhs:t): Prop :=
-    | splits_intro
-        (MSG:
-           forall to msg
-             (LHS: lhs.(messages) to = Some msg),
-             rhs.(messages) to = Some msg)
-        (OWN: lhs.(ownership) = rhs.(ownership))
+    Inductive add (cell1:t) (from to:Time.t) (msg:Message.t): forall (rhs:t), Prop :=
+    | add_intro
+        (DISJOINT: forall to2 from2 msg2
+                     (GET2: DOMap.find to2 cell1 = Some (from2, msg2)),
+            to <> from2 /\ Interval.disjoint (from, to) (from2, to2))
+        (TO1: Time.lt from to):
+        add cell1 from to msg (DOMap.add to (from, msg) cell1)
     .
 
-    Global Program Instance splits_PreOrder: PreOrder splits.
-    Next Obligation.
-      ii. econs; i; eauto.
-    Qed.
-    Next Obligation.
-      ii. inv H. inv H0. econs; auto.
-      i. rewrite OWN. auto.
-    Qed.
-
-    Lemma splits_disjoint a b a'
-          (DISJOINT: disjoint a b)
-          (SPLITS: splits a a'):
-      disjoint a' b.
+    Lemma add_wf
+          cell1 from to msg rhs
+          (ADD: add cell1 from to msg rhs)
+          (CELL1: wf cell1):
+      wf rhs.
     Proof.
-      inv SPLITS. econs. i.
-      inv DISJOINT. eapply DISJOINT0; eauto.
-      congruence.
+      inv ADD. inv CELL1. econs; i.
+      - rewrite DOMap.Facts.add_o in *.
+        destruct (DOMap.Facts.eq_dec to to0).
+        + inv GET. auto.
+        + eapply VOLUME. eauto.
+      - rewrite DOMap.Facts.add_o in *.
+        destruct (DOMap.Facts.eq_dec to to1),
+                 (DOMap.Facts.eq_dec to to2); repeat subst.
+        + congruence.
+        + inv GET1. eapply DISJOINT; eauto.
+        + inv GET2. symmetry. eapply DISJOINT; eauto.
+        + eapply DISJOINT0; eauto.
     Qed.
 
-    Lemma splits_disjoint_inv a b a'
-          (DISJOINT: disjoint a' b)
-          (SPLITS: splits a a'):
-      disjoint a b.
+    Inductive split (cell1:t) (from to1 to2:Time.t) (msg1:Message.t): forall (rhs:t), Prop :=
+    | split_intro
+        msg2
+        (GET2: DOMap.find to2 cell1 = Some (from, msg2))
+        (TO1: Time.lt from to1)
+        (TO2: Time.lt to1 to2):
+        split cell1 from to1 to2 msg1
+              (DOMap.add to1 (from, msg1) (DOMap.add to2 (to1, msg2) cell1))
+    .
+
+    Lemma split_wf
+          cell1 from1 to1 to2 msg1 cell2
+          (SPLIT: split cell1 from1 to1 to2 msg1 cell2)
+          (CELL1: wf cell1):
+      wf cell2.
     Proof.
-      inv SPLITS. econs. i.
-      inv DISJOINT. eapply DISJOINT0; eauto.
-      congruence.
-    Qed.
-
-    Lemma splits_join a b a' b'
-          (WFA: wf a)
-          (WFB: wf b)
-          (WFA': wf a')
-          (WFB': wf b')
-          (SPLITSA: splits a a')
-          (SPLITSB: splits b b')
-          (DISJOINT: disjoint a b):
-      splits (join a b) (join a' b').
-    Proof.
-      inv SPLITSA. inv SPLITSB. econs; s; i.
-      - destruct (messages a to) eqn:A, (messages b to) eqn:B,
-                 (messages a' to) eqn:A', (messages b' to) eqn:B';
-          inv LHS;
-          try (erewrite MSG in *; [|by eauto]);
-          try (erewrite MSG0 in *; [|by eauto]);
-          try inv A'; try inv B'; eauto.
-        + exfalso. eapply DISJOINT.
-          * inv WFA. eauto.
-          * inv WFB'. rewrite OWN0 in *. eauto.
-        + exfalso. eapply DISJOINT.
-          * inv WFA'. rewrite OWN in *. eauto.
-          * inv WFB. eauto.
-      - rewrite OWN, OWN0. auto.
-    Unshelve.
-    { apply Message.elt. }
-    { apply Message.elt. }
-    Qed.
-
-    Lemma splits_join_inv1 a b c
-          (WFA: wf a)
-          (WFB: wf b)
-          (WFC: wf c)
-          (SPLITS: splits (join a b) c)
-          (DISJOINT: disjoint a b):
-      exists a' b',
-        <<WFA': wf a'>> /\
-        <<WFB': wf b'>> /\
-        <<SPLITSA: splits a a'>> /\
-        <<SPLITSB: splits b b'>> /\
-        <<JOINC: c = join a' b'>>.
-    Proof.
-      exists (mk (fun t => if a.(ownership) t then c.(messages) t else None)
-            (a.(ownership))).
-      exists (mk (fun t => if b.(ownership) t then c.(messages) t else None)
-            (b.(ownership))).
-      inv SPLITS. splits.
-      - econs; s; i.
-        + destruct (ownership a ts); inv H. auto.
-        + inv WFA. exploit OWN0; eauto. i. des.
-          exists to. inv x. econs; eauto. s. rewrite OWN1.
-          * apply MSG. s. rewrite MSG1.
-            instantiate (1 := match messages b to with
-                              | Some _ => Message.elt
-                              | None => msg
-                              end).
-            destruct (messages b to); auto.
-          * apply Interval.mem_ub. inv TS. ss.
-            eapply TimeFacts.lt_le_lt; eauto.
-        + inv WFC. des. exists tos. i.
-          destruct (ownership a ts) eqn:O; inv H.
-          eapply FINITE. eauto.
-      - econs; s; i.
-        + destruct (ownership b ts); inv H. auto.
-        + inv WFB. exploit OWN0; eauto. i. des.
-          exists to. inv x. econs; eauto. s. rewrite OWN1.
-          * apply MSG. s. rewrite MSG1.
-            instantiate (1 := match messages a to with
-                              | Some _ => Message.elt
-                              | None => msg
-                              end).
-            destruct (messages a to); auto.
-          * apply Interval.mem_ub. inv TS. ss.
-            eapply TimeFacts.lt_le_lt; eauto.
-        + inv WFC. des. exists tos. i.
-          destruct (ownership b ts) eqn:O; inv H.
-          eapply FINITE. eauto.
-      - econs; auto. s. i.
-        destruct (ownership a to) eqn:O.
-        + apply MSG. s. rewrite LHS. destruct (messages b to) eqn:B; auto.
-          exfalso. eapply (@disjoint_messages a b); eauto.
-        + destruct WFA. exploit MSG0; eauto. i. congruence.
-      - econs; auto. s. i.
-        destruct (ownership b to) eqn:O.
-        + apply MSG. s. rewrite LHS. destruct (messages a to) eqn:A; auto.
-          exfalso. eapply (@disjoint_messages a b); eauto.
-        + destruct WFB. exploit MSG0; eauto. i. congruence.
-      - apply extensionality. s. i. splits.
-        + destruct (ownership a to) eqn:A, (ownership b to) eqn:B, (messages c to) eqn:C; auto.
-          * exfalso. inv DISJOINT. eapply DISJOINT0; eauto.
-          * destruct WFC. exploit MSG0; eauto.
-            rewrite <- OWN. s. rewrite A, B. intuition.
-        + rewrite <- OWN. auto.
-    Qed.
-
-    Lemma splits_join_inv2 a b c d
-          (WFA: wf a)
-          (WFB: wf b)
-          (WFC: wf c)
-          (WFD: wf d)
-          (SPLITS1: splits a c)
-          (SPLITS2: splits (join a b) (join c d))
-          (DISJOINT1: disjoint a b)
-          (DISJOINT2: disjoint c d):
-      splits b d.
-    Proof.
-      inv SPLITS1. inv SPLITS2. ss. econs; i.
-      - specialize (MSG0 to msg). rewrite LHS in *.
-        destruct (messages a to) eqn:OA.
-        { exfalso. inv DISJOINT1. eapply DISJOINT.
-          - inv WFA. eauto.
-          - inv WFB. eauto.
-        }
-        specialize (MSG0 eq_refl).
-        destruct (messages c to) eqn:OC; auto.
-        destruct (messages d to) eqn:OD.
-        { exfalso. inv DISJOINT2. eapply DISJOINT.
-          - inv WFC. eauto.
-          - inv WFD. eauto.
-        }
-        exfalso. inv DISJOINT1. eapply DISJOINT.
-        + rewrite OWN. inv WFC. eauto.
-        + inv WFB. eauto.
-      - extensionality to.
-        apply (fapp _ to) in OWN0.
-        destruct (ownership a to) eqn:OA,
-                 (ownership b to) eqn:OB,
-                 (ownership d to) eqn:OD; ss.
-        + exfalso. inv DISJOINT1. eapply DISJOINT; eauto.
-        + rewrite OWN in OA.
-          exfalso. inv DISJOINT2. eapply DISJOINT; eauto.
-        + rewrite <- OWN, OA in OWN0. ss.
-        + rewrite <- OWN, OA in OWN0. ss.
-    Qed.
-
-    Lemma join2_cancel
-          a b c
-          (A: wf a)
-          (B: wf b)
-          (C: wf c)
-          (AB: disjoint a b)
-          (AC: disjoint a c)
-          (EQ: join a b = join a c):
-      b = c.
-    Proof.
-      apply extensionality. i.
-      apply extensionality_inv in EQ. des.
-      specialize (MSG to). specialize (OWN to). ss. splits.
-      - destruct (messages a to) eqn:MA,
-                 (messages b to) eqn:MB; auto.
-        { exfalso. inv AB. eapply DISJOINT; eauto.
-          - inv A. eauto.
-          - inv B. eauto.
-        }
-        destruct (messages c to) eqn:MC; auto. inv MSG.
-        exfalso. inv AC. eapply DISJOINT; eauto.
-        + inv A. eauto.
-        + inv C. eauto.
-      - destruct (ownership a to) eqn:OA; ss.
-        destruct (ownership b to) eqn:OB,
-                 (ownership c to) eqn:OC; auto.
-        + exfalso. inv AB. eapply DISJOINT; eauto.
-        + exfalso. inv AC. eapply DISJOINT; eauto.
-    Qed.
-
-    Lemma join2_splits_lemma
-          a b c d
-          (A: wf a)
-          (B: wf b)
-          (C: wf c)
-          (D: wf d)
-          (AB: disjoint a b)
-          (CD: disjoint c d)
-          (AC: splits a c)
-          (EQ: join a b = join c d):
-      a = c.
-    Proof.
-      apply extensionality. i.
-      apply extensionality_inv in EQ. des.
-      specialize (MSG to). specialize (OWN to). ss. splits.
-      - destruct (messages a to) eqn:MA.
-        { inv AC. exploit MSG0; eauto. }
-        destruct (messages c to) eqn:MC; auto.
-        destruct (messages b to) eqn:MB.
-        { exfalso. inv AB. eapply DISJOINT.
-          - inv AC. rewrite OWN0. inv C. eauto.
-          - inv B. eauto.
-        }
-        destruct (messages d to) eqn:MD; inv MSG.
-      - inv AC. rewrite OWN0. auto.
-    Qed.
-
-    Lemma join2_inv_lemma1
-          a b c d
-          (A: wf a)
-          (B: wf b)
-          (C: wf c)
-          (D: wf d)
-          (AB: disjoint a b)
-          (CD: disjoint c d)
-          (AC: disjoint a c)
-          (EQ: join a b = join c d):
-      <<OAD: a.(ownership) <1= d.(ownership)>> /\
-      <<MAD: forall ts, a.(ownership) ts -> d.(messages) ts = a.(messages) ts>> /\
-      <<OWN: forall ts, a.(ownership) ts = andb (d.(ownership) ts) (negb (b.(ownership) ts))>>.
-    Proof.
-      apply extensionality_inv in EQ. des. splits; ss; i.
-      - specialize (OWN x0). des. rewrite PR in *. ss.
-        destruct (ownership c x0) eqn:CO; ss.
-        exfalso. inv AC. eapply DISJOINT; eauto.
-      - specialize (MSG ts).
-        destruct (messages b ts) eqn:MB.
-        { exfalso. inv AB. eapply DISJOINT; eauto.
-          inv B. eapply MSG0; eauto.
-        }
-        destruct (messages c ts) eqn:MC.
-        { exfalso. inv AC. eapply DISJOINT; eauto.
-          inv C. eapply MSG0; eauto.
-        }
-        rewrite <- MSG.
-        destruct (messages a ts); auto.
-      - specialize (OWN ts).
-        destruct (ownership a ts) eqn:OA,
-                 (ownership b ts) eqn:OB,
-                 (ownership c ts) eqn:OC,
-                 (ownership d ts) eqn:OD; ss.
-        + exfalso. inv AB. eapply DISJOINT; eauto.
-        + exfalso. inv AB. eapply DISJOINT; eauto.
-        + exfalso. inv AB. eapply DISJOINT; eauto.
-        + exfalso. inv AC. eapply DISJOINT; eauto.
-    Qed.
-
-    Lemma join2_inv_lemma2
-          a b c d
-          (A: wf a)
-          (B: wf b)
-          (C: wf c)
-          (D: wf d)
-          (AB: disjoint a b)
-          (CD: disjoint c d)
-          (AC: disjoint a c)
-          (EQ: join a b = join c d):
-      exists e, <<WF: wf e>> /\
-           <<DISJOINT: disjoint a e>> /\
-           <<D: d = join a e>>.
-    Proof.
-      Ltac tac :=
-        repeat
-          (try match goal with
-               | [H: andb _ _ = true |- _] =>
-                 apply Bool.andb_true_iff in H; des
-               | [H: is_true (andb _ _) |- _] =>
-                 apply Bool.andb_true_iff in H; des
-               | [H: andb _ _ = false |- _] =>
-                 apply Bool.andb_false_iff in H; des
-               | [H: (negb _) = true |- _] =>
-                 apply Bool.negb_true_iff in H
-               | [H: (negb _) = false |- _] =>
-                 apply Bool.negb_false_iff in H
-
-               | [H: context[if ?c then _ else _] |- _] =>
-                 let X := fresh "X" in
-                 destruct c eqn:X
-               | [H: context[match (?c):option _ with | Some _ => _ | None => _ end] |- _] =>
-                 let X := fresh "X" in
-                 destruct c eqn:X
-               | [|- context[if ?c then _ else _]] =>
-                 let X := fresh "X" in
-                 destruct c eqn:X
-               | [|- context[match (?c):option _ with | Some _ => _ | None => _ end]] =>
-                 let X := fresh "X" in
-                 destruct c eqn:X
-               end;
-           ss; subst).
-
-      exploit (@join2_inv_lemma1 a b c d); eauto; i; des.
-      exploit (@join2_inv_lemma1 c d a b); eauto; i; des.
-      { symmetry. auto. }
-      exists (mk (fun ts => if andb (d.(ownership) ts) (negb (a.(ownership) ts))
-                    then d.(messages) ts
-                    else None)
-            (fun ts => andb (d.(ownership) ts) (negb (a.(ownership) ts)))).
-      splits.
-      - econs; i; tac.
-        + generalize OWN. i. specialize (OWN1 ts). rewrite H, H0 in OWN1. ss.
-          symmetry in OWN1. apply Bool.negb_false_iff in OWN1.
-          inv B. exploit OWN2; eauto. i. des.
-          inv D. exploit OWN3; eauto. i. des.
-          inv x. inv x0.
-          destruct (TimeFacts.le_lt_dec to to0).
-          * exists to. econs.
-            { instantiate (1 := Time.join from from0).
-              inv TS. inv TS0. econs; s; eauto. ss.
-              apply TimeFacts.join_spec_lt; auto.
-            }
-            { i. inv PR. ss. apply Bool.andb_true_iff.
-              rewrite OWN.
-              admit.
-            }
-            { admit. }
-          * admit.
-        + inv D. des. exists tos. i. tac. eapply FINITE. eauto.
-      - econs; i; tac. congruence.
-      - apply extensionality. i. tac.
-        + inv A. exploit MSG; eauto. congruence.
-        + inv A. exploit MSG; eauto. congruence.
-        + inv A. exploit MSG; eauto. i. apply OAD in x. congruence.
-        + rewrite OAD, MAD, X, X1; auto.
-        + rewrite X0, X1. auto.
-        + rewrite X0.
-          destruct (messages d to) eqn:Y.
-          { inv D. exploit MSG; eauto. congruence. }
-          destruct (ownership a to) eqn:Z; auto.
-          apply OAD in Z. congruence.
-        + rewrite OAD, MAD, X, X0; auto.
+      inv SPLIT. inv CELL1. econs; i.
+      - rewrite ? DOMap.Facts.add_o in *.
+        destruct (DOMap.Facts.eq_dec to1 to).
+        { inv GET. auto. }
+        destruct (DOMap.Facts.eq_dec to2 to).
+        { inv GET. auto. }
+        eapply VOLUME. eauto.
+      - rewrite ? DOMap.Facts.add_o in *.
+        destruct (DOMap.Facts.eq_dec to1 to0),
+                 (DOMap.Facts.eq_dec to1 to3),
+                 (DOMap.Facts.eq_dec to2 to0),
+                 (DOMap.Facts.eq_dec to2 to3);
+          (repeat subst);
+          (try congruence);
+          (repeat match goal with
+                 | [H: Some _ = Some _ |- _] => inv H
+                  end);
+          (try by eapply DISJOINT; eauto).
+        + admit.
+        + ii. eapply (DISJOINT to3 to2); eauto.
+          admit.
+        + symmetry.
+          admit.
+        + ii. eapply (DISJOINT to0 to2); eauto.
+          admit.
+        + ii. eapply (DISJOINT to3 to0); eauto.
+          admit.
+        + ii. eapply (DISJOINT to0 to3); eauto.
+          admit.
     Admitted.
-
-    Lemma join2_splits
-          a b c d
-          (A: wf a)
-          (B: wf b)
-          (C: wf c)
-          (D: wf d)
-          (AB: disjoint a b)
-          (CD: disjoint c d)
-          (AC: splits a c)
-          (EQ: join a b = join c d):
-      a = c /\ b = d.
-    Proof.
-      exploit (@join2_splits_lemma a b c d); eauto. i. subst.
-      splits; auto. eapply join2_cancel; eauto.
-    Qed.
-
-    Lemma join2_inv
-          a b c d
-          (A: wf a)
-          (B: wf b)
-          (C: wf c)
-          (D: wf d)
-          (AB: disjoint a b)
-          (CD: disjoint c d)
-          (AC: disjoint a c)
-          (EQ: join a b = join c d):
-      exists e, <<WF: wf e>> /\
-           <<AE: disjoint a e>> /\
-           <<CE: disjoint c e>> /\
-           <<B: b = join c e>> /\
-           <<D: d = join a e>>.
-    Proof.
-      exploit (@join2_inv_lemma2 a b c d); eauto. i. des. subst.
-      apply join_disjoint in CD. des.
-      exists e. splits; eauto.
-      rewrite join_assoc, (join_comm _ a), <- join_assoc in EQ.
-      apply join2_cancel in EQ; auto.
-      - apply join_wf; auto.
-      - apply join_disjoint. splits; auto.
-    Qed.
   End Raw.
 
   Structure t := mk {
@@ -904,32 +629,25 @@ Module Cell.
     WF: Raw.wf raw;
   }.
 
-  Definition get (ts:Time.t) (cell:t): option Message.t := cell.(Raw.messages) ts.
-
-  Lemma extensionality
-        (cell1 cell2:t)
-        (RAW: cell1.(raw) = cell2.(raw)):
-    cell1 = cell2.
+  Lemma ext
+        (lhs rhs:t)
+        (EXT: lhs.(raw) = rhs.(raw)):
+    lhs = rhs.
   Proof.
-    destruct cell1, cell2. ss. subst.
-    assert (WF0 = WF1) by apply proof_irrelevance; subst.
-    auto.
+    destruct lhs, rhs. ss. subst.
+    f_equal. apply proof_irrelevance.
   Qed.
 
-  Lemma extensionality'
-        (cell1 cell2:t)
-        (MSG: forall to, cell1.(Raw.messages) to = cell2.(Raw.messages) to)
-        (OWN: forall to, cell1.(Raw.ownership) to = cell2.(Raw.ownership) to):
-    cell1 = cell2.
-  Proof.
-    apply extensionality. destruct cell1, cell2. ss.
-    apply Raw.extensionality; auto.
-  Qed.
+  Definition get (ts:Time.t) (cell:t): option Message.t := Raw.get ts cell.
 
-  Lemma extensionality_inv lhs rhs (EQ: lhs = rhs):
-    raw lhs = raw rhs.
-  Proof.
-    destruct lhs, rhs. inv EQ. auto.
+  Definition le (lhs rhs:t): Prop := Raw.le lhs rhs.
+
+  Global Program Instance le_PreOrder: PreOrder le.
+  Next Obligation.
+    unfold le. ii. reflexivity.
+  Qed.
+  Next Obligation.
+    unfold le. ii. etrans; eauto.
   Qed.
 
   Definition disjoint (lhs rhs:t): Prop := Raw.disjoint lhs rhs.
@@ -939,173 +657,44 @@ Module Cell.
     unfold disjoint in *. symmetry. auto.
   Qed.
 
-  Definition join (lhs rhs:t): t := @mk (Raw.join lhs rhs) (Raw.join_wf lhs.(WF) rhs.(WF)).
-
-  Lemma join_comm lhs rhs:
-    join lhs rhs = join rhs lhs.
+  Lemma disjoint_get
+        lhs rhs
+        ts lmsg rmsg
+        (DISJOINT: disjoint lhs rhs)
+        (LMSG: get ts lhs = Some lmsg)
+        (RMSG: get ts rhs = Some rmsg):
+    False.
   Proof.
-    apply extensionality. apply Raw.join_comm.
+    destruct lmsg, rmsg. unfold get, Raw.get in *.
+    destruct (DOMap.find ts lhs.(raw)) as [[]|] eqn:LHS; inv LMSG.
+    destruct (DOMap.find ts rhs.(raw)) as [[]|] eqn:RHS; inv RMSG.
+    eapply DISJOINT; eauto.
+    - apply Interval.mem_ub. eapply WF. eauto.
+    - apply Interval.mem_ub. eapply WF. eauto.
   Qed.
 
-  Lemma join_assoc a b c:
-    join a (join b c) = join (join a b) c.
-  Proof.
-    apply extensionality. apply Raw.join_assoc.
-  Qed.
+  Definition bot: t := mk Raw.bot_wf.
 
-  Lemma join_disjoint a b c:
-    disjoint a (join b c) <-> disjoint a b /\ disjoint a c.
-  Proof.
-    apply Raw.join_disjoint.
-  Qed.
+  Lemma bot_le cell: le bot cell.
+  Proof. apply Raw.bot_le. Qed.
 
-  Definition bot: t := @mk Raw.bot Raw.bot_wf.
-
-  Lemma bot_disjoint cell: disjoint cell bot.
+  Lemma bot_disjoint cell: disjoint bot cell.
   Proof. apply Raw.bot_disjoint. Qed.
-
-  Lemma bot_join cell: join cell bot = cell.
-  Proof.
-    apply extensionality. apply Raw.bot_join.
-  Qed.
-
-  Lemma bot_join_inv a b
-        (EQ: a = join a b)
-        (DISJOINT: disjoint a b):
-    b = bot.
-  Proof.
-    apply extensionality.
-    eapply Raw.bot_join_inv; try apply WF; eauto.
-    apply extensionality_inv in EQ. auto.
-  Qed.
 
   Definition singleton
              (from to:Time.t) (msg:Message.t)
              (LT: Time.lt from to): t :=
-    @mk (Raw.singleton from to msg) (Raw.singleton_wf msg LT).
+    mk (Raw.singleton_wf msg LT).
 
   Definition init: t :=
-    @singleton (Time.decr Time.elt)
-               Time.elt
-               (Message.mk 0 Capability.elt)
-               (Time.decr_spec Time.elt).
+    singleton (Message.mk 0 Capability.elt)
+              (Time.decr_spec Time.elt).
 
-  Definition splits (lhs rhs:t): Prop := Raw.splits lhs rhs.
+  Definition add (cell1:t) (from1 to1:Time.t) (msg1:Message.t) (cell2:t): Prop :=
+    Raw.add cell1 from1 to1 msg1 cell2.
 
-  Global Program Instance splits_PreOrder: PreOrder splits.
-  Next Obligation.
-    ii. unfold splits in *. reflexivity.
-  Qed.
-  Next Obligation.
-    ii. unfold splits in *. etrans; eauto.
-  Qed.
-
-  Lemma splits_disjoint a b a'
-        (DISJOINT: disjoint a b)
-        (SPLITS: splits a a'):
-    disjoint a' b.
-  Proof.
-    eapply Raw.splits_disjoint; eauto.
-  Qed.
-
-  Lemma splits_disjoint_inv a b a'
-        (DISJOINT: disjoint a' b)
-        (SPLITS: splits a a'):
-    disjoint a b.
-  Proof.
-    eapply Raw.splits_disjoint_inv; eauto.
-  Qed.
-
-  Lemma splits_join a b a' b'
-        (SPLITSA: splits a a')
-        (SPLITSB: splits b b')
-        (DISJOINT: disjoint a b):
-    splits (join a b) (join a' b').
-  Proof.
-    exploit (@Raw.splits_join a b a' b'); eauto; apply WF.
-  Qed.
-
-  Lemma splits_join_inv1 a b c
-        (SPLITS: splits (join a b) c)
-        (DISJOINT: disjoint a b):
-    exists a' b',
-      <<SPLITSA: splits a a'>> /\
-      <<SPLITSB: splits b b'>> /\
-      <<JOINC: c = join a' b'>>.
-  Proof.
-    destruct a as [a WFA], b as [b WFB], c as [c WFC].
-    unfold disjoint, splits in *. ss.
-    exploit (@Raw.splits_join_inv1 a b c); eauto. i. des. subst.
-    exists (@mk a' WFA'), (@mk b' WFB'). splits; eauto.
-    apply extensionality. auto.
-  Qed.
-
-  Lemma splits_join_inv2 a b c d
-        (SPLITS1: splits a c)
-        (SPLITS2: splits (join a b) (join c d))
-        (DISJOINT1: disjoint a b)
-        (DISJOINT2: disjoint c d):
-    splits b d.
-  Proof.
-    destruct a as [a WFA], b as [b WFB], c as [c WFC], d as [d WFD].
-    unfold disjoint, splits in *. ss.
-    exploit (@Raw.splits_join_inv2 a b c d); eauto.
-  Qed.
-
-  Lemma join2_cancel
-        a b c
-        (AB: disjoint a b)
-        (AC: disjoint a c)
-        (EQ: join a b = join a c):
-    b = c.
-  Proof.
-    exploit (@Raw.join2_cancel a b c);
-      try apply WF;
-      try apply AB;
-      try apply AC.
-    - apply extensionality_inv in EQ. auto.
-    - i. des. splits; apply extensionality; auto.
-  Qed.
-
-  Lemma join2_splits
-        a b c d
-        (AB: disjoint a b)
-        (CD: disjoint c d)
-        (AC: splits a c)
-        (EQ: join a b = join c d):
-    a = c /\ b = d.
-  Proof.
-    exploit (@Raw.join2_splits a b c d);
-      try apply WF;
-      try apply AB;
-      try apply CD;
-      try apply AC.
-    - apply extensionality_inv in EQ. auto.
-    - i. des. splits; apply extensionality; auto.
-  Qed.
-
-  Lemma join2_inv
-        a b c d
-        (AB: disjoint a b)
-        (CD: disjoint c d)
-        (AC: disjoint a c)
-        (EQ: join a b = join c d):
-    exists e, <<AE: disjoint a e>> /\
-         <<CE: disjoint c e>> /\
-         <<B: b = join c e>> /\
-         <<D: d = join a e>>.
-  Proof.
-    exploit (@Raw.join2_inv a b c d);
-      try apply WF;
-      try apply AB;
-      try apply CD;
-      try apply AC.
-    - apply extensionality_inv in EQ. auto.
-    - i. des.
-      exists (@mk e WF0). splits; auto.
-      + apply extensionality. auto.
-      + apply extensionality. auto.
-  Qed.
+  Definition split (cell1:t) (from1 to1 to2:Time.t) (msg1:Message.t) (cell2:t): Prop :=
+    Raw.split cell1 from1 to1 to2 msg1 cell2.
 End Cell.
 
 Module Memory.
@@ -1114,27 +703,16 @@ Module Memory.
   Definition get (loc:Loc.t) (ts:Time.t) (mem:t): option Message.t :=
     Cell.get ts (mem loc).
 
-  Inductive wf_timemap (times:TimeMap.t) (mem:t): Prop :=
-  | wf_timemap_intro
-      (WF: forall loc, exists ts msg,
-            <<TS: Time.le (times loc) ts>> /\
-            <<MSG: get loc ts mem = Some msg>>)
-  .
+  Definition le (lhs rhs:t): Prop :=
+    forall loc, Cell.le (lhs loc) (rhs loc).
 
-  Inductive wf_capability (capability:Capability.t) (mem:t): Prop :=
-  | wf_capability_intro
-      (UR: wf_timemap capability.(Capability.ur) mem)
-      (RW: wf_timemap capability.(Capability.rw) mem)
-      (SC: wf_timemap capability.(Capability.sc) mem)
-      (UR_RW: TimeMap.le capability.(Capability.ur) capability.(Capability.rw))
-      (RW_SC: TimeMap.le capability.(Capability.rw) capability.(Capability.sc))
-  .
-
-  Inductive wf (mem:t): Prop :=
-  | wf_intro
-      (WF: forall loc ts msg (MSG: get loc ts mem = Some msg),
-          wf_capability msg.(Message.released) mem)
-  .
+  Global Program Instance le_PreOrder: PreOrder le.
+  Next Obligation.
+    ii. reflexivity.
+  Qed.
+  Next Obligation.
+    ii. etrans; eauto.
+  Qed.
 
   Inductive disjoint (lhs rhs:t): Prop :=
   | disjoint_intro
@@ -1142,398 +720,181 @@ Module Memory.
   .
 
   Global Program Instance disjoint_Symmetric: Symmetric disjoint.
-  Next Obligation. econs. ii. symmetry. apply H. Qed.
-
-  Definition join (lhs rhs:t): t := fun loc => Cell.join (lhs loc) (rhs loc).
-
-  Lemma join_comm lhs rhs:
-    join lhs rhs = join rhs lhs.
-  Proof. extensionality i. apply Cell.join_comm. Qed.
-
-  Lemma join_assoc a b c:
-    join a (join b c) = join (join a b) c.
-  Proof. extensionality i. apply Cell.join_assoc. Qed.
-
-  Lemma join_disjoint a b c:
-    disjoint a (join b c) <-> disjoint a b /\ disjoint a c.
-  Proof.
-    econs; i; des; splits; econs; i.
-    - inv H. specialize (DISJOINT loc). apply Cell.join_disjoint in DISJOINT. des. auto.
-    - inv H. specialize (DISJOINT loc). apply Cell.join_disjoint in DISJOINT. des. auto.
-    - inv H. inv H0. apply Cell.join_disjoint. splits; auto.
+  Next Obligation.
+    econs. ii. symmetry. apply H.
   Qed.
 
-  Lemma join_get
-        a b loc ts msg
-        (DISJOINT: disjoint a b)
-        (GET: get loc ts a = Some msg):
-    get loc ts (join a b) = Some msg.
-  Proof.
-    unfold get, Cell.get, join, Cell.join in *. ss.
-    destruct (Cell.Raw.messages (Cell.raw (a loc)) ts) eqn:A,
-             (Cell.Raw.messages (Cell.raw (b loc)) ts) eqn:B;
-      inv GET; auto.
-    exfalso. eapply DISJOINT; eapply Cell.WF; eauto.
-  Qed.
+  Definition bot: t := fun _ => Cell.bot.
 
-  Lemma join_get_None
-        a b loc ts
-        (DISJOINT: disjoint a b)
-        (GETA: get loc ts a = None)
-        (GETB: get loc ts b = None):
-    get loc ts (join a b) = None.
-  Proof.
-    unfold get, Cell.get, join, Cell.join in *. ss.
-    destruct (Cell.Raw.messages (Cell.raw (a loc)) ts) eqn:A,
-             (Cell.Raw.messages (Cell.raw (b loc)) ts) eqn:B;
-      inv GETA; inv GETB; auto.
-  Qed.
+  Lemma bot_le mem: le bot mem.
+  Proof. ii. apply Cell.bot_le. Qed.
 
-  Lemma join_get_inv
-        a b loc ts msg
-        (DISJOINT: disjoint a b)
-        (GET: get loc ts (join a b) = Some msg):
-    get loc ts a = Some msg \/ get loc ts b = Some msg.
-  Proof.
-    unfold get, Cell.get, join, Cell.join in *. ss.
-    destruct (Cell.Raw.messages (Cell.raw (a loc)) ts) eqn:A,
-             (Cell.Raw.messages (Cell.raw (b loc)) ts) eqn:B;
-      inv GET; auto.
-    exfalso. eapply DISJOINT; eapply Cell.WF; eauto.
-  Qed.
-
-  Lemma join_get_None_inv
-        a b loc ts
-        (DISJOINT: disjoint a b)
-        (GET: get loc ts (join a b) = None):
-    get loc ts a = None /\ get loc ts b = None.
-  Proof.
-    unfold get, Cell.get, join, Cell.join in *. ss.
-    destruct (Cell.Raw.messages (Cell.raw (a loc)) ts) eqn:A,
-             (Cell.Raw.messages (Cell.raw (b loc)) ts) eqn:B;
-      inv GET; auto.
-  Qed.
-
-  Definition bot: t := LocFun.init Cell.bot.
-
-  Lemma bot_disjoint mem: disjoint mem bot.
-  Proof. econs. ii. apply Cell.bot_disjoint. Qed.
-
-  Lemma bot_join mem: join mem bot = mem.
-  Proof.
-    extensionality loc. apply Cell.bot_join.
-  Qed.
-
-  Lemma bot_join_inv a b
-        (EQ: a = join a b)
-        (DISJOINT: disjoint a b):
-    b = bot.
-  Proof.
-    inversion DISJOINT.
-    extensionality loc. eapply Cell.bot_join_inv; eauto.
-    apply (fapp _ loc) in EQ. auto.
-  Qed.
+  Lemma bot_disjoint mem: disjoint bot mem.
+  Proof. econs. i. apply Cell.bot_disjoint. Qed.
 
   Definition singleton
              (loc:Loc.t) (from to:Time.t) (msg:Message.t)
              (LT: Time.lt from to): t :=
-    (LocFun.add loc (@Cell.mk (Cell.Raw.singleton from to msg) (Cell.Raw.singleton_wf msg LT))
-                (LocFun.init Cell.bot)).
+    (LocFun.add loc (Cell.mk (Cell.Raw.singleton_wf msg LT))
+                (fun _ => Cell.bot)).
 
-  Lemma singleton_get
-        loc from to msg
-        (LT: Time.lt from to):
-    get loc to (singleton loc msg LT) = Some msg.
-  Proof.
-    unfold get, singleton, LocFun.add.
-    destruct (Loc.eq_dec loc loc); [|congruence].
-    unfold Cell.get. ss.
-    destruct (Time.eq_dec to to); [|congruence]. auto.
-  Qed.
+  Definition init: t := fun _ => Cell.init.
 
-  Lemma singleton_get_inv
-        loc1 ts1 msg1
-        loc2 from2 to2 msg2 (LT2: Time.lt from2 to2)
-        (GET: get loc1 ts1 (singleton loc2 msg2 LT2) = Some msg1):
-    loc1 = loc2 /\ ts1 = to2 /\ msg1 = msg2.
-  Proof.
-    unfold singleton, get, Cell.get, LocFun.add, LocFun.find in *.
-    destruct (Loc.eq_dec loc1 loc2); ss. subst.
-    destruct (Time.eq_dec ts1 to2); inv GET. auto.
-  Qed.
+  Definition closed_timemap (times:TimeMap.t) (mem:t): Prop :=
+    forall loc, exists ts msg,
+        <<TS: Time.le (times loc) ts>> /\
+        <<MSG: get loc ts mem = Some msg>>.
 
-  Definition init: t := LocFun.init Cell.init.
-
-  Definition splits (lhs rhs:t): Prop := forall loc, Cell.splits (lhs loc) (rhs loc).
-
-  Global Program Instance splits_PreOrder: PreOrder splits.
-  Next Obligation. ii. reflexivity. Qed.
-  Next Obligation. ii. etrans; eauto. Qed.
-
-  Lemma splits_get a b
-        loc ts msg
-        (SIM: splits a b)
-        (TGT: get loc ts a = Some msg):
-    get loc ts b = Some msg.
-  Proof.
-    unfold get, Cell.get in *.
-    apply SIM. auto.
-  Qed.
-
-  Lemma splits_disjoint a b a'
-        (DISJOINT: disjoint a b)
-        (SPLITS: splits a a'):
-    disjoint a' b.
-  Proof.
-    inv DISJOINT. econs. ii. eapply Cell.splits_disjoint; eauto.
-  Qed.
-
-  Lemma splits_disjoint_inv a b a'
-        (DISJOINT: disjoint a' b)
-        (SPLITS: splits a a'):
-    disjoint a b.
-  Proof.
-    inv DISJOINT. econs. ii. eapply Cell.splits_disjoint_inv; eauto.
-  Qed.
-
-  Lemma splits_intro
-        loc from to to0 msg msg0
-        (LT1: Time.lt from to)
-        (LT2: Time.lt to to0):
-    <<SPLIT: splits (singleton loc msg0 (TimeSet.Raw.MX.lt_trans LT1 LT2))
-                    (join (singleton loc msg LT1) (singleton loc msg0 LT2))>> /\
-    <<DISJOINT: disjoint (singleton loc msg LT1) (singleton loc msg0 LT2)>>.
-  Proof.
-    splits.
-    - unfold singleton, LocFun.add, LocFun.find. econs; s; i.
-      + destruct (Loc.eq_dec loc0 loc); ss. subst.
-        destruct (Time.eq_dec to1 to); ss. subst.
-        destruct (Time.eq_dec to to0); ss. subst.
-        apply Time.lt_strorder in LT2. done.
-      + destruct (Loc.eq_dec loc0 loc); ss. subst.
-        extensionality ts.
-        destruct (TimeFacts.le_lt_dec ts from); ss.
-        * destruct (TimeFacts.le_lt_dec ts to); ss.
-          destruct (TimeFacts.le_lt_dec ts to0); ss.
-          exploit (@TimeFacts.le_lt_lt ts from to); auto. i.
-          rewrite x0 in l0. apply Time.lt_strorder in l0. done.
-        * destruct (TimeFacts.le_lt_dec ts to0),
-          (TimeFacts.le_lt_dec ts to); ss.
-          exploit (@TimeFacts.le_lt_lt ts to to0); auto. i.
-          rewrite x0 in l0. apply Time.lt_strorder in l0. done.
-    - unfold singleton, LocFun.add, LocFun.find. econs. ii. econs. ii.
-      destruct (Loc.eq_dec loc0 loc); ss. subst.
-      destruct (TimeFacts.le_lt_dec ts from); ss.
-      destruct (TimeFacts.le_lt_dec ts to); ss.
-  Qed.
-
-  Lemma splits_join a b a' b'
-        (SPLITSA: splits a a')
-        (SPLITSB: splits b b')
-        (DISJOINT: disjoint a b):
-    splits (join a b) (join a' b').
-  Proof.
-    inv DISJOINT. ii. apply Cell.splits_join; auto.
-  Qed.
-
-  Lemma splits_join_inv1 a b c
-        (SPLITS: splits (join a b) c)
-        (DISJOINT: disjoint a b):
-    exists a' b',
-      <<SPLITSA: splits a a'>> /\
-      <<SPLITSB: splits b b'>> /\
-      <<JOINC: c = join a' b'>>.
-  Proof.
-    inv DISJOINT.
-    exploit (@choice Loc.t (Cell.t * Cell.t)
-                     (fun loc ab =>
-                        <<SPLITSA: Cell.splits (a loc) ab.(fst)>> /\
-                        <<SPLITSB: Cell.splits (b loc) ab.(snd)>> /\
-                        <<JOINC: (c loc) = Cell.join ab.(fst) ab.(snd)>>)).
-    - i. exploit Cell.splits_join_inv1; eauto. i. des.
-      eexists (_, _). splits; eauto.
-    - i. des.
-      exists (fun loc => (f loc).(fst)), (fun loc => (f loc).(snd)). splits.
-      + ii. specialize (x0 loc). des. auto.
-      + ii. specialize (x0 loc). des. auto.
-      + extensionality loc. specialize (x0 loc). des. auto.
-  Qed.
-
-  Lemma splits_join_inv2 a b c d
-        (SPLITS1: splits a c)
-        (SPLITS2: splits (join a b) (join c d))
-        (DISJOINT1: disjoint a b)
-        (DISJOINT2: disjoint c d):
-    splits b d.
-  Proof.
-    inv DISJOINT1. inv DISJOINT2.
-    ii. eapply Cell.splits_join_inv2; eauto.
-  Qed.
-
-  Lemma join2_cancel
-        a b c
-        (AB: disjoint a b)
-        (AC: disjoint a c)
-        (EQ: join a b = join a c):
-    b = c.
-  Proof.
-    inv AB. inv AC.
-    extensionality loc. eapply Cell.join2_cancel; eauto.
-    apply (fapp _ loc) in EQ. auto.
-  Qed.
-
-  Lemma join2_splits
-        a b c d
-        (AB: disjoint a b)
-        (CD: disjoint c d)
-        (AC: splits a c)
-        (EQ: join a b = join c d):
-    a = c /\ b = d.
-  Proof.
-    splits.
-    - extensionality loc.
-      exploit Cell.join2_splits.
-      + apply AB.
-      + apply CD.
-      + apply AC.
-      + apply (fapp _ loc) in EQ. eauto.
-      + i. des. auto.
-    - extensionality loc.
-      exploit Cell.join2_splits.
-      + apply AB.
-      + apply CD.
-      + apply AC.
-      + apply (fapp _ loc) in EQ. eauto.
-      + i. des. auto.
-  Qed.
-
-  Lemma join2_inv
-        a b c d
-        (AB: disjoint a b)
-        (CD: disjoint c d)
-        (AC: disjoint a c)
-        (EQ: join a b = join c d):
-    exists e, <<AE: disjoint a e>> /\
-         <<CE: disjoint c e>> /\
-         <<B: b = join c e>> /\
-         <<D: d = join a e>>.
-  Proof.
-    inv AB. inv CD. inv AC.
-    exploit (@choice Loc.t Cell.t
-                     (fun loc e =>
-                        <<AE: Cell.disjoint (a loc) e>> /\
-                        <<CE: Cell.disjoint (c loc) e>> /\
-                        <<B: b loc = Cell.join (c loc) e>> /\
-                        <<D: d loc = Cell.join (a loc) e>>)).
-    - i. exploit (@Cell.join2_inv (a x) (b x) (c x) (d x)); eauto.
-      eapply (fapp _ x) in EQ. ss.
-    - i. des. exists f. splits.
-      + econs. intro loc. exploit x0; eauto. i. des. eauto.
-      + econs. intro loc. exploit x0; eauto. i. des. eauto.
-      + extensionality loc. exploit x0; eauto. i. des. eauto.
-      + extensionality loc. exploit x0; eauto. i. des. eauto.
-  Qed.
-
-  Inductive le (lhs rhs:t): Prop :=
-  | le_intro
-      ohs
-      (JOIN: join lhs ohs = rhs)
-      (DISJOINT: disjoint lhs ohs)
+  Inductive closed_capability (capability:Capability.t) (mem:t): Prop :=
+  | closed_capability_intro
+      (UR: closed_timemap capability.(Capability.ur) mem)
+      (RW: closed_timemap capability.(Capability.rw) mem)
+      (SC: closed_timemap capability.(Capability.sc) mem)
   .
 
-  Global Program Instance le_PreOrder: PreOrder le.
-  Next Obligation.
-    ii. econs.
-    - apply bot_join.
-    - apply bot_disjoint.
-  Qed.
-  Next Obligation.
-    ii. inv H. inv H0. econs.
-    - apply join_assoc.
-    - symmetry in DISJOINT0. apply join_disjoint in DISJOINT0. des.
-      apply join_disjoint. splits; [eauto|].
-      symmetry. eauto.
-  Qed.
+  Definition closed (mem:t): Prop :=
+    forall loc ts msg (MSG: get loc ts mem = Some msg),
+      <<WF: Capability.wf msg.(Message.released)>> /\
+      <<CLOSED: closed_capability msg.(Message.released) mem>>.
 
-  Lemma le_get
-        loc ts msg mem1 mem2
-        (LE: le mem1 mem2)
-        (GET: get loc ts mem1 = Some msg):
-    get loc ts mem2 = Some msg.
-  Proof.
-    inv LE. unfold get, join, Cell.get, Cell.join in *. ss.
-    rewrite GET.
-    destruct (Cell.Raw.messages (Cell.raw (ohs loc)) ts) eqn:B; auto.
-    exfalso. eapply DISJOINT; eapply Cell.WF; eauto.
-  Qed.
+  Definition closed_promises (promises:Promises.t) (mem:t): Prop :=
+    forall loc ts (PROMISES: Promises.mem loc ts promises),
+    exists msg, get loc ts mem = Some msg.
 
-  Lemma le_join_l lhs rhs
-        (DISJOINT: disjoint lhs rhs):
-    le lhs (join lhs rhs).
-  Proof. econs; eauto. Qed.
-
-  Lemma le_join_r lhs rhs
-        (DISJOINT: disjoint lhs rhs):
-    le rhs (join lhs rhs).
-  Proof. symmetry in DISJOINT. rewrite join_comm. econs; eauto. Qed.
-
-  Lemma le_join a b c d
-        (AB: disjoint a b)
-        (CD: disjoint c d)
-        (AC: le a c)
-        (BD: le b d):
-    le (join a b) (join c d).
-  Proof.
-    inv AC. inv BD.
-    rewrite <- ? join_assoc, (join_assoc ohs b ohs0).
-    rewrite (join_comm ohs b), ? join_assoc.
-    apply join_disjoint in CD. des.
-    symmetry in CD. apply join_disjoint in CD. des.
-    symmetry in CD0. apply join_disjoint in CD0. des.
-    etrans; [|apply le_join_l].
-    - apply le_join_l.
-      symmetry. apply join_disjoint. splits; symmetry; auto.
-    - symmetry. apply join_disjoint. splits; auto.
-      apply join_disjoint. splits; auto.
-      symmetry. auto.
-  Qed.
-
-  (* TODO: define future as the transitive closure of add/split operations *)
-  Inductive future (lhs rhs:t): Prop :=
-  | future_intro
-      lhs'
-      (SPLITS: splits lhs lhs')
-      (LE: le lhs' rhs):
-      future lhs rhs
+  Inductive add (mem1:t) (loc:Loc.t) (from1 to1:Time.t) (msg1:Message.t): forall (mem2:t), Prop :=
+  | add_intro
+      r
+      (ADD: Cell.add (mem1 loc) from1 to1 msg1 r)
+      (WF: Capability.wf msg1.(Message.released))
+      (CLOSED: closed_capability msg1.(Message.released) (LocFun.add loc r mem1)):
+      add mem1 loc from1 to1 msg1 (LocFun.add loc r mem1)
   .
 
-  Global Program Instance future_PreOrder: PreOrder future.
-  Next Obligation.
-    ii. econs; reflexivity.
-  Qed.
-  Next Obligation.
-    ii. inv H. inv H0. inv LE. inv LE0.
-    exploit (@splits_join_inv1 lhs' ohs lhs'0); eauto. i. des. subst.
-    rewrite <- join_assoc. econs.
-    - etrans; eauto.
-    - apply le_join_l.
-      symmetry in DISJOINT0. apply join_disjoint in DISJOINT0. des.
-      apply join_disjoint. splits.
-      + eapply splits_disjoint; [|eauto].
-        symmetry. eapply splits_disjoint; [|eauto].
-        symmetry. auto.
-      + symmetry. auto.
-  Qed.
+  Inductive split (mem1:t) (loc:Loc.t) (from1 to1 to2:Time.t) (msg1:Message.t): forall (mem2:t), Prop :=
+  | split_intro
+      r
+      (SPLIT: Cell.split (mem1 loc) from1 to1 to2 msg1 r)
+      (WF: Capability.wf msg1.(Message.released))
+      (CLOSED: closed_capability msg1.(Message.released) (LocFun.add loc r mem1)):
+      split mem1 loc from1 to1 to2 msg1 (LocFun.add loc r mem1)
+  .
 
-  Lemma le_future: le <2= future.
-  Proof.
-    i. econs; eauto. reflexivity.
-  Qed.
+  Inductive future_imm (mem1 mem2:t): Prop :=
+  | future_imm_add
+      loc from1 to1 msg1
+      (ADD: add mem1 loc from1 to1 msg1 mem2)
+  | future_imm_split
+      loc from1 to1 to2 msg1
+      (SPLIT: split mem1 loc from1 to1 to2 msg1 mem2)
+  .
+
+  Inductive splits_imm (mem1 mem2:t): Prop :=
+  | splits_imm_intro
+      loc from1 to1 to2 msg1
+      (SPLIT: split mem1 loc from1 to1 to2 msg1 mem2)
+  .
+
+  Definition future := rtc future_imm.
+  Definition splits := rtc splits_imm.
 
   Lemma splits_future: splits <2= future.
   Proof.
-    i. econs; eauto. reflexivity.
+    i. induction PR.
+    - econs 1.
+    - econs 2; eauto. inv H. econs 2. eauto.
   Qed.
+
+  Inductive promise
+            (promises1:Promises.t) (mem1:t)
+            (loc:Loc.t) (from1 to1:Time.t) (msg1:Message.t):
+    forall (promises2:Promises.t) (mem2:t), Prop :=
+  | promise_add
+      mem2
+      (ADD: add mem1 loc from1 to1 msg1 mem2):
+      promise promises1 mem1 loc from1 to1 msg1 (Promises.set loc to1 promises1) mem2
+  | promise_split
+      to2 mem2
+      (SPLIT: split mem1 loc from1 to1 to2 msg1 mem2)
+      (OWN: Promises.mem loc to2 promises1):
+      promise promises1 mem1 loc from1 to1 msg1 (Promises.set loc to1 promises1) mem2
+  .
+
+  Inductive fulfill
+            (promises1:Promises.t) (mem1:t)
+            (loc:Loc.t) (to:Time.t) (msg:Message.t):
+    forall (promises2:Promises.t), Prop :=
+  | fulfill_intro
+      (GET: get loc to mem1 = Some msg)
+      (OWN: Promises.mem loc to promises1):
+      fulfill promises1 mem1 loc to msg (Promises.unset loc to promises1)
+  .
+
+
+  (* Lemmas on add & split *)
+
+  Lemma add_get1
+        mem1 loc from1 to1 msg1 mem2
+        l t m
+        (ADD: add mem1 loc from1 to1 msg1 mem2)
+        (GET: get l t mem1 = Some m):
+    get l t mem2 = Some m.
+  Proof.
+  Admitted.
+
+  Lemma add_get2
+        mem1 loc from1 to1 msg1 mem2
+        (ADD: add mem1 loc from1 to1 msg1 mem2):
+    get loc to1 mem2 = Some msg1.
+  Proof.
+  Admitted.
+
+  Lemma add_disjoint
+        mem1 loc from1 to1 msg1 mem2
+        (ADD: add mem1 loc from1 to1 msg1 mem2):
+    get loc to1 mem1 = None.
+  Proof.
+  Admitted.
+
+  Lemma add_get_inv
+        mem1 loc from1 to1 msg1 mem2
+        l t m
+        (ADD: add mem1 loc from1 to1 msg1 mem2)
+        (GET: get l t mem2 = Some m):
+    (l = loc /\ t = to1 /\ m = msg1) \/ get l t mem1 = Some m.
+  Proof.
+  Admitted.
+
+  Lemma split_get1
+        mem1 loc from1 to1 to2 msg1 mem2
+        l t m
+        (ADD: split mem1 loc from1 to1 to2 msg1 mem2)
+        (GET: get l t mem1 = Some m):
+    get l t mem2 = Some m.
+  Proof.
+  Admitted.
+
+  Lemma split_get2
+        mem1 loc from1 to1 to2 msg1 mem2
+        (ADD: split mem1 loc from1 to1 to2 msg1 mem2):
+    get loc to1 mem2 = Some msg1.
+  Proof.
+  Admitted.
+
+  Lemma split_disjoint
+        mem1 loc from1 to1 to2 msg1 mem2
+        (SPLIT: split mem1 loc from1 to1 to2 msg1 mem2):
+    get loc to1 mem1 = None.
+  Proof.
+  Admitted.
+
+  Lemma split_get_inv
+        mem1 loc from1 to1 to2 msg1 mem2
+        l t m
+        (SPLIT: split mem1 loc from1 to1 to2 msg1 mem2)
+        (GET: get l t mem2 = Some m):
+    (l = loc /\ t = to1 /\ m = msg1) \/ get l t mem1 = Some m.
+  Proof.
+  Admitted.
 
   Lemma future_get
         loc ts msg mem1 mem2
@@ -1541,409 +902,212 @@ Module Memory.
         (GET: get loc ts mem1 = Some msg):
     get loc ts mem2 = Some msg.
   Proof.
-    inv LE. eapply le_get; eauto. eapply splits_get; eauto.
+    induction LE; auto. apply IHLE. inv H.
+    - eapply add_get1; eauto.
+    - eapply split_get1; eauto.
   Qed.
 
-  Lemma future_wf_timemap
-        times mem1 mem2
-        (WF: wf_timemap times mem1)
-        (FUTURE: future mem1 mem2):
-    wf_timemap times mem2.
+  Lemma splits_get
+        loc ts msg mem1 mem2
+        (LE: splits mem1 mem2)
+        (GET: get loc ts mem1 = Some msg):
+    get loc ts mem2 = Some msg.
   Proof.
-    inv WF. econs. i. specialize (WF0 loc). des.
-    inv FUTURE. exploit splits_get; eauto. i.
-    inv LE. unfold get, join, Cell.get, Cell.join in *. s.
-    eexists _. rewrite x0. destruct (Cell.Raw.messages (Cell.raw (ohs loc)) ts); eauto.
+    induction LE; auto. apply IHLE.
+    inv H. eapply split_get1; eauto.
   Qed.
 
-  Lemma future_wf_capability
-        capability mem1 mem2
-        (WF: wf_capability capability mem1)
-        (FUTURE: future mem1 mem2):
-    wf_capability capability mem2.
-  Proof.
-    inv WF. econs; eauto.
-    - eapply future_wf_timemap; eauto.
-    - eapply future_wf_timemap; eauto.
-    - eapply future_wf_timemap; eauto.
-  Qed.
 
-  Lemma incr_wf_timemap
-        loc s ts msg mem
-        (WF1: wf_timemap s mem)
-        (WF2: get loc ts mem = Some msg):
-    wf_timemap (TimeMap.incr loc ts s) mem.
-  Proof.
-    unfold TimeMap.incr, LocFun.add, LocFun.find. econs. i.
-    destruct (Loc.eq_dec loc0 loc).
-    - subst.
-      destruct (Time.join_cases (s loc) ts) as [X|X]; rewrite X; eauto.
-      + apply WF1.
-      + eexists _, _. splits; eauto. reflexivity.
-    - apply WF1.
-  Qed.
+  (* Lemmas on closedness *)
 
-  Lemma join_wf_timemap
+  Lemma join_closed_timemap
         lhs rhs mem
-        (LHS: wf_timemap lhs mem)
-        (RHS: wf_timemap rhs mem):
-    wf_timemap (TimeMap.join lhs rhs) mem.
+        (LHS: closed_timemap lhs mem)
+        (RHS: closed_timemap rhs mem):
+    closed_timemap (TimeMap.join lhs rhs) mem.
   Proof.
-    econs. i. unfold TimeMap.join.
+    ii. unfold TimeMap.join.
     destruct (Time.join_cases (lhs loc) (rhs loc)) as [X|X]; rewrite X.
     - apply LHS.
     - apply RHS.
   Qed.
 
-  Lemma wf_capability_join
+  Lemma join_closed_capability
         lhs rhs mem
-        (LHS: wf_capability lhs mem)
-        (RHS: wf_capability rhs mem):
-    wf_capability (Capability.join lhs rhs) mem.
+        (LHS: closed_capability lhs mem)
+        (RHS: closed_capability rhs mem):
+    closed_capability (Capability.join lhs rhs) mem.
   Proof.
     econs.
-    - apply join_wf_timemap.
+    - apply join_closed_timemap.
       + apply LHS.
       + apply RHS.
-    - apply join_wf_timemap.
+    - apply join_closed_timemap.
       + apply LHS.
       + apply RHS.
-    - apply join_wf_timemap.
+    - apply join_closed_timemap.
       + apply LHS.
       + apply RHS.
-    - apply TimeMap.join_spec.
-      + etrans; [apply LHS|]. apply TimeMap.join_l.
-      + etrans; [apply RHS|]. apply TimeMap.join_r.
-    - apply TimeMap.join_spec.
-      + etrans; [apply LHS|]. apply TimeMap.join_l.
-      + etrans; [apply RHS|]. apply TimeMap.join_r.
   Qed.
 
-  Lemma wf_incr_ur
-        loc ts s msg mem
-        (WF: wf_capability s mem)
-        (GET: get loc ts mem = Some msg):
-    wf_capability (Capability.incr_ur loc ts s) mem.
+  Lemma future_closed_timemap
+        times mem1 mem2
+        (CLOSED: closed_timemap times mem1)
+        (FUTURE: future mem1 mem2):
+    closed_timemap times mem2.
   Proof.
-    inv WF. econs; s.
-    - eapply incr_wf_timemap; eauto.
-    - eapply incr_wf_timemap; eauto.
-    - eapply incr_wf_timemap; eauto.
-    - apply TimeMap.incr_mon. auto.
-    - apply TimeMap.incr_mon. auto.
+    ii. exploit CLOSED; eauto. i. des.
+    eexists _, _. splits; eauto. eapply future_get; eauto.
   Qed.
 
-  Lemma wf_incr_rw
-        loc ts s msg mem
-        (WF: wf_capability s mem)
-        (GET: get loc ts mem = Some msg):
-    wf_capability (Capability.incr_rw loc ts s) mem.
+  Lemma future_closed_capability
+        capability mem1 mem2
+        (CLOSED: closed_capability capability mem1)
+        (FUTURE: future mem1 mem2):
+    closed_capability capability mem2.
   Proof.
-    inv WF. econs; s.
+    inv CLOSED. econs; eauto.
+    - eapply future_closed_timemap; eauto.
+    - eapply future_closed_timemap; eauto.
+    - eapply future_closed_timemap; eauto.
+  Qed.
+
+  Lemma future_closed_promises
+        promises mem1 mem2
+        (CLOSED: closed_promises promises mem1)
+        (FUTURE: future mem1 mem2):
+    closed_promises promises mem2.
+  Proof.
+    ii. exploit CLOSED; eauto. i. des.
+    eexists. eapply future_get; eauto.
+  Qed.
+
+  Lemma incr_closed_timemap
+        loc s ts msg mem
+        (CLOSED: closed_timemap s mem)
+        (GET: get loc ts mem = Some msg):
+    closed_timemap (TimeMap.incr loc ts s) mem.
+  Proof.
+    unfold TimeMap.incr, LocFun.add, LocFun.find. ii.
+    destruct (Loc.eq_dec loc0 loc).
+    - destruct (Time.join_cases (s loc) ts) as [X|X]; rewrite X; eauto.
+      + exploit CLOSED. i. des.
+        eexists _, _. splits; eauto. subst. eauto.
+      + eexists _, _. splits; eauto. reflexivity. subst loc. eauto.
+    - apply CLOSED.
+  Qed.
+
+  Lemma incr_ur_closed_capability
+        loc ts s msg mem
+        (CLOSED: closed_capability s mem)
+        (GET: get loc ts mem = Some msg):
+    closed_capability (Capability.incr_ur loc ts s) mem.
+  Proof.
+    inv CLOSED. econs; s.
+    - eapply incr_closed_timemap; eauto.
+    - eapply incr_closed_timemap; eauto.
+    - eapply incr_closed_timemap; eauto.
+  Qed.
+
+  Lemma incr_rw_closed_capability
+        loc ts s msg mem
+        (CLOSED: closed_capability s mem)
+        (GET: get loc ts mem = Some msg):
+    closed_capability (Capability.incr_rw loc ts s) mem.
+  Proof.
+    inv CLOSED. econs; s.
     - auto.
-    - eapply incr_wf_timemap; eauto.
-    - eapply incr_wf_timemap; eauto.
-    - etrans; [apply TimeMap.incr_le|].
-      apply TimeMap.incr_mon. auto.
-    - apply TimeMap.incr_mon. auto.
+    - eapply incr_closed_timemap; eauto.
+    - eapply incr_closed_timemap; eauto.
   Qed.
 
-  Ltac tac :=
-    repeat
-      (try match goal with
-           | [H: le _ _ |- _] =>
-             inv H
-           | [H: disjoint _ (join _ _) |- _] =>
-             apply join_disjoint in H
-           | [H: disjoint (join _ _) _ |- _] =>
-             symmetry in H; apply join_disjoint in H
-           | [H1: ?a = join ?a ?b, H2: disjoint ?a ?b |- _] =>
-             apply bot_join_inv in H1; [|apply H2]
-           | [H1: ?a = join ?a ?b, H2: disjoint ?b ?a |- _] =>
-             apply bot_join_inv in H1; [|symmetry; apply H2]
-           | [H: disjoint ?a ?b |- disjoint ?b ?a] =>
-             symmetry
-           | [H1: disjoint ?a ?b, H2: splits ?a ?a' |- disjoint ?a' ?b] =>
-             eapply (@splits_disjoint a b a'); eauto
-           | [H1: disjoint ?a ?b, H2: splits ?a ?a' |- disjoint ?b ?a'] =>
-             symmetry; eapply (@splits_disjoint a b a'); eauto
-           | [H1: disjoint ?b ?a, H2: splits ?a ?a' |- disjoint ?a' ?b] =>
-             symmetry in H1; eapply (@splits_disjoint a b a'); eauto
-           | [H1: disjoint ?b ?a, H2: splits ?a ?a' |- disjoint ?b ?a'] =>
-             symmetry; symmetry in H1; eapply (@splits_disjoint a b a'); eauto
-           | [H: join ?a ?b = join ?a ?c |- _] =>
-             apply join2_cancel in H; [|clear H|clear H]
-           | [|- disjoint _ (join _ _)] =>
-             apply join_disjoint
-           | [|- disjoint (join _ _) _] =>
-             symmetry; apply join_disjoint
 
-           | [H1: disjoint ?a ?b, H2: get _ _ (join ?a ?b) = Some _ |- _] =>
-             apply join_get_inv in H2; auto
-           | [H1: disjoint ?a ?b, H2: get _ _ (join ?a ?b) = None |- _] =>
-             apply join_get_None_inv in H2; auto
-           end;
-       ss; des; try subst; auto).
-
-  Inductive promise
-            (promise1 global1:t)
-            (loc:Loc.t) (from to:Time.t) (msg:Message.t)
-            (promise2:t) (global2:t): Prop :=
-  | promise_add
-      (LT: Time.lt from to)
-      (DISJOINT: disjoint global1 (singleton loc msg LT))
-      (PROMISEEQ: promise2 = join promise1 (singleton loc msg LT))
-      (GLOBALEQ: global2 = join global1 (singleton loc msg LT))
-      (WF: wf_capability msg.(Message.released) global2)
-  | promise_split
-      promise1_ctx global1_ctx to0 msg0
-      (LT1: Time.lt from to)
-      (LT2: Time.lt to to0)
-      (PROMISE1: promise1 = join promise1_ctx (singleton loc msg0 (TimeSet.Raw.MX.lt_trans LT1 LT2)))
-      (PROMISE2: disjoint promise1_ctx (singleton loc msg0 (TimeSet.Raw.MX.lt_trans LT1 LT2)))
-      (GLOBAL1: global1 = join global1_ctx promise1)
-      (GLOBAL2: disjoint global1_ctx promise1)
-      (PROMISEEQ: promise2 = join promise1_ctx (join (singleton loc msg LT1) (singleton loc msg0 LT2)))
-      (GLOBALEQ: global2 = join global1_ctx (join promise1_ctx (join (singleton loc msg LT1) (singleton loc msg0 LT2))))
-      (WF: wf_capability msg.(Message.released) global2)
-  .
+  (* Lemmas on promise & fulfill *)
 
   Lemma promise_future
-        promise1 global1 loc from to msg promise2 global2
-        (LE1: le promise1 global1)
-        (WF1: wf global1)
-        (PROMISE: promise promise1 global1 loc from to msg promise2 global2):
-    <<LE2: le promise2 global2>> /\
-    <<WF2: wf global2>> /\
-    <<FUTURE: future global1 global2>>.
+        promises1 mem1 loc from to msg promises2 mem2
+        (CLOSED_PROMISES1: closed_promises promises1 mem1)
+        (CLOSED1: closed mem1)
+        (PROMISE: promise promises1 mem1 loc from to msg promises2 mem2):
+    <<CLOSED_PROMISES2: closed_promises promises2 mem2>> /\
+    <<CLOSED2: closed mem2>> /\
+    <<FUTURE: future mem1 mem2>>.
   Proof.
-    inv PROMISE; tac.
+    inv PROMISE.
     - splits.
-      + econs.
-        * rewrite <- join_assoc, (join_comm (singleton loc msg LT)), join_assoc. tac.
-        * repeat (splits; tac).
-      + inv WF1. econs. i.
-        apply join_get_inv in MSG; [|tac]. des.
-        * exploit WF0; eauto. i.
-          eapply future_wf_capability; eauto.
-          apply le_future. apply le_join_l. tac.
-        * apply singleton_get_inv in MSG. des. subst. auto.
-      + apply le_future. econs; tac.
-    - rewrite ? join_assoc, (join_comm global1_ctx _), <- ? join_assoc in JOIN. tac.
-      + generalize (splits_intro loc msg msg0 LT1 LT2). intro SPLIT.
-        rewrite (join_comm global1_ctx _) in JOIN. tac. splits.
-        * apply le_join_r. repeat (splits; tac).
-        * admit. (* memory wf *)
-        * apply splits_future. repeat (apply splits_join; tac).
-      + repeat (splits; tac).
-      + repeat (splits; tac).
-  Admitted.
+      + ii. apply Promises.set_inv in PROMISES. des.
+        * subst. eexists. eapply add_get2. eauto.
+        * exploit CLOSED_PROMISES1; eauto. i. des.
+          eexists. eapply add_get1; eauto.
+      + ii. eapply add_get_inv in MSG; eauto. des.
+        * subst. inv ADD. eauto.
+        * exploit CLOSED1; eauto. i. des. splits; auto.
+          eapply future_closed_capability; eauto.
+          econs 2; eauto. econs 1. eauto.
+      + econs 2; eauto. econs 1. eauto.
+    - splits.
+      + ii. apply Promises.set_inv in PROMISES. des.
+        * subst. eexists. eapply split_get2. eauto.
+        * exploit CLOSED_PROMISES1; eauto. i. des.
+          eexists. eapply split_get1; eauto.
+      + ii. eapply split_get_inv in MSG; eauto. des.
+        * subst. inv SPLIT. eauto.
+        * exploit CLOSED1; eauto. i. des. splits; auto.
+          eapply future_closed_capability; eauto.
+          econs 2; eauto. econs 2. eauto.
+      + econs 2; eauto. econs 2. eauto.
+  Qed.
 
   Lemma promise_disjoint
-        promise1 global1 loc from to msg promise2 global2 ctx
-        (LE1: le promise1 global1)
-        (LE2: le ctx global1)
-        (DISJOINT1: disjoint promise1 ctx)
-        (PROMISE: promise promise1 global1 loc from to msg promise2 global2):
-    <<DISJOINT2: disjoint promise2 ctx>> /\
-    <<LE2: le ctx global2>>.
-  Proof.
-    inv PROMISE; tac.
-    - apply join2_inv in JOIN; tac. splits.
-      + repeat (splits; tac).
-      + rewrite <- join_assoc. apply le_join_l.
-        repeat (splits; tac).
-    - rewrite ? join_assoc, (join_comm global1_ctx _), <- ? join_assoc in JOIN0.
-      generalize (splits_intro loc msg msg0 LT1 LT2). intro SPLIT.
-      repeat (splits; tac).
-      rewrite (join_comm global1_ctx _) in JOIN0. tac.
-      rewrite ? join_assoc, (join_comm global1_ctx _), <- ? join_assoc in JOIN.
-      apply join2_inv in JOIN; repeat (splits; tac).
-      rewrite (join_comm global1_ctx _) in D.
-      apply join2_inv in D; repeat (splits; tac).
-      rewrite <- join_assoc. apply le_join_l. repeat (splits; tac).
-  Qed.
-
-  Lemma disjoint_get
-        lhs rhs loc to msgl msgr
-        (DISJOINT: disjoint lhs rhs)
-        (LHS: get loc to lhs = Some msgl)
-        (RHS: get loc to rhs = Some msgr):
-    False.
-  Proof.
-    inv DISJOINT. eapply DISJOINT0.
-    - eapply Cell.WF. eauto.
-    - eapply Cell.WF. eauto.
-  Qed.
-
-  Lemma disjoint_get_None
-        lhs rhs loc to msgl
-        (DISJOINT: disjoint lhs rhs)
-        (LHS: get loc to lhs = Some msgl):
-    get loc to rhs = None.
-  Proof.
-    destruct (get loc to rhs) eqn:RHS; auto.
-    exfalso. eapply disjoint_get; eauto.
-  Qed.
-
-  Lemma promise_get1 promise1 global1 loc from to msg promise2 global2
-        (LE: le promise1 global1)
-        (PROMISE: promise promise1 global1 loc from to msg promise2 global2):
-    get loc to global1 = None.
-  Proof.
-    destruct (get loc to global1) eqn:MSG1; auto.
-    inv PROMISE.
-    - exfalso. eapply disjoint_get; eauto.
-      apply singleton_get.
-    - generalize (splits_intro loc msg msg0 LT1 LT2). i. des.
-      exploit splits_disjoint.
-      { symmetry. apply GLOBAL2. }
-      { apply splits_join. reflexivity. eauto. tac. }
-      i. tac.
-      exploit splits_disjoint.
-      { symmetry. apply PROMISE2. }
-      { apply SPLIT. }
-      i. tac.
-      apply join_get_inv in MSG1; (splits; tac).
-      + exfalso. eapply disjoint_get; try apply x1; eauto.
-        apply singleton_get.
-      + exfalso. eapply disjoint_get; try apply x3; eauto.
-        apply singleton_get.
-      + apply singleton_get_inv in MSG1. des. subst.
-        exfalso. eapply Time.lt_strorder. eauto.
-  Qed.
-
-  Lemma promise_get2 promise1 global1 loc from to msg promise2 global2
-        (LE: le promise1 global1)
-        (PROMISE: promise promise1 global1 loc from to msg promise2 global2):
-    get loc to global2 = Some msg.
+        promises1 mem1 loc from to msg promises2 mem2 ctx
+        (CLOSED_PROMISES1: closed_promises promises1 mem1)
+        (WF1: closed mem1)
+        (PROMISE: promise promises1 mem1 loc from to msg promises2 mem2)
+        (CLOSED_PROMISES: closed_promises ctx mem1)
+        (DISJOINT: Promises.disjoint promises1 ctx):
+    Promises.disjoint promises2 ctx.
   Proof.
     inv PROMISE.
-    - rewrite join_comm. apply join_get; repeat (splits; tac).
-      apply singleton_get.
-    - generalize (splits_intro loc msg msg0 LT1 LT2). i. des.
-      exploit splits_disjoint.
-      { symmetry. apply GLOBAL2. }
-      { apply splits_join. reflexivity. eauto. tac. }
-      i. tac.
-      rewrite join_comm. apply join_get; repeat (splits; tac).
-      rewrite join_comm. apply join_get; repeat (splits; tac).
-      apply join_get; repeat (splits; tac).
-      apply singleton_get.
+    - econs. i. apply Promises.set_inv in LHS. des.
+      + subst. exploit CLOSED_PROMISES; eauto. i. des.
+        exploit add_disjoint; eauto. congruence.
+      + eapply DISJOINT; eauto.
+    - econs. i. apply Promises.set_inv in LHS. des.
+      + subst. exploit CLOSED_PROMISES; eauto. i. des.
+        exploit split_disjoint; eauto. congruence.
+      + eapply DISJOINT; eauto.
   Qed.
-
-  Lemma promise_get_inv promise1 global1 loc from to msg promise2 global2
-        loc' to' msg'
-        (LE: le promise1 global1)
-        (PROMISE: promise promise1 global1 loc from to msg promise2 global2)
-        (GET: get loc' to' promise2 = Some msg'):
-    get loc' to' promise1 = Some msg' \/
-    loc = loc' /\ to = to' /\ msg = msg'.
-  Proof.
-    inv PROMISE.
-    - apply join_get_inv in GET; tac.
-      apply singleton_get_inv in GET. des. auto.
-    - generalize (splits_intro loc msg msg0 LT1 LT2). i. des.
-      exploit splits_disjoint.
-      { symmetry. apply GLOBAL2. }
-      { apply splits_join. reflexivity. eauto. tac. }
-      i. tac.
-      exploit splits_disjoint.
-      { symmetry. apply PROMISE2. }
-      { apply SPLIT. }
-      i. tac.
-      apply join_get_inv in GET; repeat (splits; tac).
-      + left. apply join_get; repeat (splits; tac).
-      + apply singleton_get_inv in GET. des. auto.
-      + apply singleton_get_inv in GET. des. subst.
-        left. rewrite join_comm.
-        apply join_get; repeat (splits; tac).
-        apply singleton_get.
-  Qed.
-
-  Inductive fulfill (promise1:t) (loc:Loc.t) (from to:Time.t) (msg:Message.t): forall (promise2:t), Prop :=
-  | fulfill_intro
-      promise1_ctx
-      (LT: Time.lt from to)
-      (PROMISE1: promise1 = join promise1_ctx (singleton loc msg LT))
-      (PROMISE2: disjoint promise1_ctx (singleton loc msg LT)):
-      fulfill promise1 loc from to msg promise1_ctx
-  .
 
   Lemma fulfill_future
-        promise1 global loc from to msg promise2
-        (LE1: le promise1 global)
-        (FULFILL: fulfill promise1 loc from to msg promise2):
-    le promise2 global.
+        promises1 mem1 loc to msg promises2
+        (CLOSED_PROMISES1: closed_promises promises1 mem1)
+        (WF1: closed mem1)
+        (FULFILL: fulfill promises1 mem1 loc to msg promises2):
+    closed_promises promises2 mem1.
   Proof.
-    inv FULFILL; tac.
-    rewrite <- join_assoc. apply le_join_l. repeat (splits; tac).
+    inv FULFILL. ii. apply Promises.unset_inv in PROMISES. des.
+    apply CLOSED_PROMISES1. auto.
   Qed.
 
   Lemma fulfill_disjoint
-        promise1 global loc from to msg promise2 ctx
-        (LE1: le promise1 global)
-        (LE2: le ctx global)
-        (DISJOINT1: disjoint promise1 ctx)
-        (FULFILL: fulfill promise1 loc from to msg promise2):
-    <<DISJOINT2: disjoint promise2 ctx>> /\
-    <<LE2: le ctx global>>.
+        promises1 mem1 loc to msg promises2 ctx
+        (CLOSED_PROMISES1: closed_promises promises1 mem1)
+        (WF1: closed mem1)
+        (FULFILL: fulfill promises1 mem1 loc to msg promises2)
+        (CLOSED_PROMISES: closed_promises ctx mem1)
+        (DISJOINT: Promises.disjoint promises1 ctx):
+    Promises.disjoint promises2 ctx.
   Proof.
-    inv FULFILL; tac.
-    apply join2_inv in JOIN; tac. splits.
-    - repeat (splits; tac).
-    - etrans; [|apply le_join_r]; repeat (splits; tac).
-      apply le_join_l; tac.
+    inv FULFILL. econs. i. apply Promises.unset_inv in LHS. des.
+    eapply DISJOINT; eauto.
   Qed.
 
-  Lemma fulfill_get promise1 loc from to msg promise2
-        (FULFILL: fulfill promise1 loc from to msg promise2):
-    get loc to promise1 = Some msg.
+  Lemma fulfill_mon
+        promises1 mem1 mem1' loc to msg promises2
+        (FULFILL: fulfill promises1 mem1 loc to msg promises2)
+        (FUTURE: future mem1 mem1'):
+    fulfill promises1 mem1' loc to msg promises2.
   Proof.
-    inv FULFILL. rewrite join_comm.
-    apply join_get; tac.
-    apply singleton_get.
-  Qed.
-
-  Lemma splits_antisym
-        a b
-        (AB: splits a b)
-        (BA: splits b a):
-    a = b.
-  Proof.
-    extensionality loc. unfold splits in *.
-    specialize (AB loc). specialize (BA loc).
-    inv AB. inv BA. apply Cell.extensionality'.
-    - i.
-      match goal with
-      | [|- ?a = ?b] => destruct a eqn:A
-      end.
-      { apply MSG in A. auto. }
-      match goal with
-      | [|- ?a = ?b] => destruct b eqn:B; auto
-      end.
-      apply MSG0 in B. congruence.
-    - i. rewrite OWN. auto.
-  Qed.
-
-  Lemma future_future_le_le
-        a b c
-        (AB: future a b)
-        (BC: future b c)
-        (AC: le a c):
-    le a b.
-  Proof.
-    inv AB. inv BC. tac.
-    apply splits_join_inv1 in SPLITS0; auto. des. subst. tac.
-    rewrite <- join_assoc in JOIN.
-    exploit join2_splits; try apply JOIN; repeat (splits; tac).
-    - eapply splits_disjoint; [|apply SPLITSA].
-      symmetry. eapply splits_disjoint; [|apply SPLITSB].
-      symmetry. auto.
-    - rewrite SPLITS. auto.
-    - exploit splits_antisym; eauto. i. subst.
-      apply le_join_l. tac.
+    inv FULFILL. econs; eauto. eapply future_get; eauto.
   Qed.
 End Memory.
-
-Ltac memtac := Memory.tac.
