src/opt/MemInv.v
@@ -10,6 +10,7 @@ Require Import respectful5.
 Require Import Axioms.
 Require Import Basic.
 Require Import Event.
+Require Import DenseOrder.
 Require Import Time.
 Require Import Language.
 Require Import Memory.
@@ -40,183 +41,140 @@ Proof.
 Qed.
 
 Module MemInv.
-  Definition t := Memory.t.
+  Definition t := Promises.t.
 
-  Inductive sem (inv:t): forall (promise_src promise_tgt:Memory.t), Prop :=
+  Inductive sem (inv:t) (promises_src promises_tgt:Promises.t): Prop :=
   | sem_intro
-      promise_tgt
-      (DISJOINT: Memory.disjoint promise_tgt inv):
-      sem inv (Memory.join promise_tgt inv) promise_tgt
+      (DISJOINT: Promises.disjoint promises_tgt inv)
+      (JOIN: promises_src = Promises.join inv promises_tgt)
   .
 
   Lemma promise
         inv
         loc from to msg
-        promise1_src global1_src
-        promise1_tgt global1_tgt promise2_tgt global2_tgt
-        (LE1_SRC: Memory.le promise1_src global1_src)
-        (LE1_TGT: Memory.le promise1_tgt global1_tgt)
-        (SIM1: sim_memory global1_src global1_tgt)
-        (INV1: sem inv promise1_src promise1_tgt)
-        (PROMISE_TGT: Memory.promise promise1_tgt global1_tgt loc from to msg promise2_tgt global2_tgt):
-    exists promise2_src global2_src,
-      <<LE1_SRC: Memory.le promise2_src global2_src>> /\
-      <<SIM2: sim_memory global2_src global2_tgt>> /\
-      <<INV2: sem inv promise2_src promise2_tgt>> /\
-      <<PROMISE_SRC: Memory.promise promise1_src global1_src loc from to msg promise2_src global2_src>>.
+        promises1_src mem1_src
+        promises1_tgt mem1_tgt promises2_tgt mem2_tgt
+        (PROMISES_TGT: Memory.promise promises1_tgt mem1_tgt loc from to msg promises2_tgt mem2_tgt)
+        (INV1: sem inv promises1_src promises1_tgt)
+        (SIM1: sim_memory mem1_src mem1_tgt)
+        (WF1_PROMISES_SRC: Memory.closed_promises promises1_src mem1_src)
+        (WF1_PROMISES_TGT: Memory.closed_promises promises1_tgt mem1_tgt):
+    exists promises2_src mem2_src,
+      <<PROMISES_SRC: Memory.promise promises1_src mem1_src loc from to msg promises2_src mem2_src>> /\
+      <<INV2: sem inv promises2_src promises2_tgt>> /\
+      <<WF1_PROMISES_SRC: Memory.closed_promises promises2_src mem2_src>> /\
+      <<SIM2: sim_memory mem2_src mem2_tgt>>.
   Proof.
-    inv SIM1. inv INV1. inv PROMISE_TGT; memtac.
-    - rewrite <- Memory.join_assoc in SPLITS.
-      apply Memory.splits_join_inv2 in SPLITS; repeat (splits; memtac).
-      exists (Memory.join (Memory.join promise1_tgt inv) (Memory.singleton loc msg LT)).
-      exists (Memory.join (Memory.join (Memory.join promise1_tgt inv) (Memory.singleton loc msg LT)) ohs).
-      splits.
-      + apply Memory.le_join_l. repeat (splits; memtac).
-        symmetry in DISJOINT3. eapply Memory.splits_disjoint in DISJOINT3; [|eauto].
-        memtac.
-      + econs. rewrite <- ? Memory.join_assoc.
-        apply Memory.splits_join; (repeat (splits; memtac)).
-        rewrite (Memory.join_comm _ ohs), Memory.join_assoc.
-        apply Memory.splits_join; (repeat (splits; memtac)).
-      + rewrite <- ? Memory.join_assoc, (Memory.join_comm inv _).
-        rewrite Memory.join_assoc. econs. repeat (splits; memtac).
-        symmetry in DISJOINT3. eapply Memory.splits_disjoint in DISJOINT3; [|eauto].
-        memtac.
-      + econs 1; eauto.
-        * symmetry in DISJOINT3. eapply Memory.splits_disjoint in DISJOINT3; [|eauto].
-          repeat (splits; memtac).
-        * rewrite <- (Memory.join_assoc _ (Memory.singleton _ _ _) ohs).
-          rewrite (Memory.join_comm (Memory.singleton _ _ _) ohs).
-          rewrite Memory.join_assoc.
-          auto.
-        * eapply Memory.future_wf_capability; eauto.
-          rewrite <- ? Memory.join_assoc. apply Memory.splits_future.
-          apply Memory.splits_join; repeat (splits; memtac).
-          rewrite (Memory.join_comm _ ohs). rewrite Memory.join_assoc.
-          apply Memory.splits_join; repeat (splits; memtac).
-    - rewrite Memory.join_assoc, (Memory.join_comm _ promise1_ctx) in SPLITS.
-      rewrite <- ? Memory.join_assoc in SPLITS.
-      apply Memory.splits_join_inv2 in SPLITS; repeat (splits; memtac).
-      rewrite (Memory.join_comm global1_ctx _) in SPLITS.
-      apply Memory.splits_join_inv2 in SPLITS; repeat (splits; memtac).
-      rewrite ? Memory.join_assoc, (Memory.join_comm _ promise1_ctx) in JOIN.
-      rewrite <- ? Memory.join_assoc in JOIN. repeat (splits; memtac).
-      rewrite (Memory.join_comm global1_ctx _) in JOIN. memtac.
-      generalize (Memory.splits_intro loc msg msg0 LT1 LT2). i. des.
-      exists (Memory.join (Memory.join inv promise1_ctx)
-                     (Memory.join (Memory.singleton loc msg LT1) (Memory.singleton loc msg0 LT2))).
-      exists (Memory.join (Memory.join (Memory.join inv ohs0) promise1_ctx)
-                     (Memory.join (Memory.singleton loc msg LT1) (Memory.singleton loc msg0 LT2))).
-      splits.
-      + symmetry in DISJOINT5. symmetry in PROMISE2. symmetry in DISJOINT3.
-        exploit Memory.splits_disjoint; try apply SPLIT; try apply DISJOINT5; eauto. i. memtac.
-        exploit Memory.splits_disjoint; try apply SPLIT; try apply PROMISE2; eauto. i. memtac.
-        exploit Memory.splits_disjoint; try apply SPLIT; try apply DISJOINT3; eauto. i. memtac.
-        repeat apply Memory.le_join;
-          try reflexivity;
-          repeat (splits; memtac).
-        apply Memory.le_join_l. memtac.
-      + econs. rewrite <- Memory.join_assoc.
-        apply Memory.splits_join; (repeat (splits; memtac)).
-      + rewrite <- ? Memory.join_assoc, (Memory.join_comm inv _).
-        econs. repeat (splits; memtac).
-      + econs 2.
-        * rewrite Memory.join_comm, ? Memory.join_assoc. auto.
-        * repeat (splits; memtac).
-        * instantiate (1 := ohs0).
-          rewrite ? Memory.join_assoc, (Memory.join_comm ohs0 _).
-          rewrite <- ? Memory.join_assoc. f_equal.
-          rewrite (Memory.join_comm ohs0 _).
-          rewrite ? Memory.join_assoc. auto.
-        * repeat (splits; memtac).
-        * auto.
-        * rewrite ? Memory.join_assoc, (Memory.join_comm ohs0 _). auto.
-        * admit. (* wf_capability *)
   Admitted.
 
   Lemma fulfill_tgt
-        inv promise1_src promise1_tgt promise2_tgt
-        loc from to msg
-        (INV: sem inv promise1_src promise1_tgt)
-        (FULFILL: Memory.fulfill promise1_tgt loc from to msg promise2_tgt):
-    exists (LT: Time.lt from to),
-      <<DISJOINT: Memory.disjoint inv (Memory.singleton loc msg LT)>> /\
-      <<INV: sem (Memory.join inv (Memory.singleton loc msg LT)) promise1_src promise2_tgt>>.
+        inv
+        promises1_src
+        promises1_tgt mem1_tgt promises2_tgt
+        loc to msg
+        (FULFILL_TGT: Memory.fulfill promises1_tgt mem1_tgt loc to msg promises2_tgt)
+        (INV1: sem inv promises1_src promises1_tgt):
+    <<DISJOINT: ~ Promises.mem loc to inv>> /\
+    <<INV2: sem (Promises.set loc to inv) promises1_src promises2_tgt>>.
   Proof.
-    inv INV. inv FULFILL. memtac.
-    exists LT. splits; memtac.
-    rewrite <- Memory.join_assoc, Memory.join_comm.
-    econs. memtac. splits; memtac.
-  Qed.
+    inv INV1. inv FULFILL_TGT.
+    splits.
+    - ii. eapply DISJOINT; eauto.
+    - econs.
+      + admit.
+      + admit.
+  Admitted.
 
   Lemma fulfill_src
-        inv1 inv2 promise1_src promise1_tgt
-        loc from to msg
-        (INV: sem inv1 promise1_src promise1_tgt)
-        (FULFILL: Memory.fulfill inv1 loc from to msg inv2):
-    exists (LT: Time.lt from to) promise2_src,
-      <<FULFILL: Memory.fulfill promise1_src loc from to msg promise2_src>> /\
-      <<INV: sem inv2 promise2_src promise1_tgt>>.
+        inv1 inv2
+        promises1_src mem1_src
+        promises1_tgt
+        loc to msg
+        (FULFILL_INV: Memory.fulfill inv1 mem1_src loc to msg inv2)
+        (INV1: sem inv1 promises1_src promises1_tgt):
+    exists promises2_src,
+      <<FULFILL_SRC: Memory.fulfill promises1_src mem1_src loc to msg promises2_src>> /\
+      <<INV2: sem inv2 promises2_src promises1_tgt>>.
   Proof.
-    inv INV. inv FULFILL. memtac.
-    exists LT. eexists. splits; memtac.
-    rewrite Memory.join_assoc. econs; memtac. splits; memtac.
-  Qed.
+    inv INV1. eexists. splits.
+    - inv FULFILL_INV. econs; eauto. admit.
+    - econs.
+      + admit.
+      + admit.
+  Admitted.
 
   Lemma fulfill
         inv
-        loc from to msg
-        promise1_src global1_src
-        promise1_tgt global1_tgt promise2_tgt
-        (LE1_SRC: Memory.le promise1_src global1_src)
-        (LE1_TGT: Memory.le promise1_tgt global1_tgt)
-        (SIM1: sim_memory global1_src global1_tgt)
-        (INV1: sem inv promise1_src promise1_tgt)
-        (FULFILL_TGT: Memory.fulfill promise1_tgt loc from to msg promise2_tgt):
-    exists promise2_src,
-      <<LE1_SRC: Memory.le promise2_src global1_src>> /\
-      <<INV2: sem inv promise2_src promise2_tgt>> /\
-      <<FULFILL_SRC: Memory.fulfill promise1_src loc from to msg promise2_src>>.
+        loc to msg
+        promises1_src mem1_src
+        promises1_tgt mem1_tgt promises2_tgt
+        (FULFILL_TGT: Memory.fulfill promises1_tgt mem1_tgt loc to msg promises2_tgt)
+        (INV1: sem inv promises1_src promises1_tgt)
+        (SIM1: sim_memory mem1_src mem1_tgt)
+        (WF1_PROMISES_SRC: Memory.closed_promises promises1_src mem1_src)
+        (WF1_PROMISES_TGT: Memory.closed_promises promises1_tgt mem1_tgt)
+        (WF1_SRC: Memory.closed mem1_src):
+    exists promises2_src,
+      <<FULFILL_SRC: Memory.fulfill promises1_src mem1_src loc to msg promises2_src>> /\
+      <<INV2: sem inv promises2_src promises2_tgt>> /\
+      <<WF1_PROMISES_SRC: Memory.closed_promises promises2_src mem1_src>>.
   Proof.
     exploit fulfill_tgt; eauto. i. des.
-    exploit fulfill_src; eauto.
-    { econs; eauto. }
+    exploit fulfill_src; try apply INV2; eauto.
+    { econs.
+      - inv FULFILL_TGT. eauto.
+      - rewrite Promises.set_o.
+        destruct (Loc.eq_dec loc loc); [|congruence].
+        destruct (Time.eq_dec to to); [|congruence].
+        auto.
+    }
     i. des.
-    exploit Memory.fulfill_future; try apply FULFILL; eauto.
-  Qed.
+    exploit Memory.fulfill_mon; eauto; i.
+    { apply Memory.splits_future. apply SIM1. }
+    eexists. splits; eauto.
+    - admit.
+    - eapply Memory.fulfill_future; eauto.
+  Admitted.
 
   Lemma future
         inv
-        promise_src global1_src global2_src
-        promise_tgt global1_tgt
-        (LE1_SRC: Memory.le promise_src global1_src)
-        (LE1_TGT: Memory.le promise_tgt global1_tgt)
-        (SIM1: sim_memory global1_src global1_tgt)
-        (INV1: sem inv promise_src promise_tgt)
-        (FUTURE_SRC: Memory.future global1_src global2_src)
-        (LE2_SRC: Memory.le promise_src global2_src):
-      <<FUTURE_TGT: Memory.future global1_tgt global2_src>> /\
-      <<LE2_TGT: Memory.le promise_tgt global2_src>>.
+        promises_src mem1_src mem2_src
+        promises_tgt mem1_tgt
+        (FUTURE_SRC: Memory.future mem1_src mem2_src)
+        (INV1: sem inv promises_src promises_tgt)
+        (SIM1: sim_memory mem1_src mem1_tgt)
+        (WF1_PROMISES_SRC: Memory.closed_promises promises_src mem1_src)
+        (WF1_PROMISES_TGT: Memory.closed_promises promises_tgt mem1_tgt)
+        (WF2_PROMISES_SRC: Memory.closed_promises promises_src mem2_src):
+      <<FUTURE_TGT: Memory.future mem1_tgt mem2_src>> /\
+      <<WF2_PROMISES_TGT: Memory.closed_promises promises_tgt mem2_src>>.
   Proof.
-    splits.
-    - rewrite <- FUTURE_SRC.
-      apply Memory.splits_future. inv SIM1. auto.
-    - rewrite <- LE2_SRC. inv INV1.
-      apply Memory.le_join_l. memtac.
-  Qed.
+    revert INV1 SIM1 WF1_PROMISES_SRC WF1_PROMISES_TGT WF2_PROMISES_SRC.
+    revert inv mem1_tgt promises_src promises_tgt.
+    induction FUTURE_SRC; i.
+    - splits.
+      + apply Memory.splits_future. apply SIM1.
+      + admit.
+    - inv H.
+      + admit.
+      + eapply IHFUTURE_SRC; eauto.
+        * admit.
+        * admit.
+  Admitted.
 
   Lemma sem_bot promise:
-    sem Memory.bot promise promise.
+    sem Promises.bot promise promise.
   Proof.
-    rewrite <- (Memory.bot_join promise) at 1.
-    econs. memtac.
-  Qed.
+    econs.
+    - admit.
+    - admit.
+  Admitted.
 
   Lemma sem_bot_inv
-        promise_src promise_tgt
-        (SEM: sem Memory.bot promise_src promise_tgt):
-    promise_src = promise_tgt.
+        promises_src promises_tgt
+        (SEM: sem Promises.bot promises_src promises_tgt):
+    promises_src = promises_tgt.
   Proof.
-    inv SEM. apply Memory.bot_join.
-  Qed.
+    inv SEM. admit.
+  Admitted.
 End MemInv.
