src/lang/Progress.v
@@ -21,8 +21,8 @@ Lemma internal_step_promise
       lang
       st1 lc1 mem1 st2 lc2 mem2
       (STEP: Thread.internal_step (Thread.mk lang st1 lc1 mem1) (Thread.mk lang st2 lc2 mem2))
-      (PROMISE: lc1.(Local.promise) = Memory.bot):
-  lc2.(Local.promise) = Memory.bot.
+      (PROMISES: lc1.(Local.promises) = Promises.bot):
+  lc2.(Local.promises) = Promises.bot.
 Proof.
   inv STEP; try inv LOCAL; ss.
   - admit.
@@ -40,7 +40,7 @@ Inductive max_timestamp (loc:Loc.t) (ts:Time.t) (mem:Memory.t): Prop :=
 
 Lemma exists_max_timestamp
       loc mem
-      (WF: Memory.wf mem):
+      (WF: Memory.closed mem):
   exists ts, max_timestamp loc ts mem.
 Proof.
 Admitted.
@@ -58,16 +58,15 @@ Lemma progress_promise_step
       (MAX: max_timestamp loc from mem1)
       (LT: Time.lt from to)
       (WF1: Local.wf lc1 mem1):
-  exists promise2 mem2,
-    Local.promise_step lc1 mem1 loc from to val released (Local.mk lc1.(Local.commit) promise2) mem2.
+  exists promises2 mem2,
+    Local.promise_step lc1 mem1 loc from to val released (Local.mk lc1.(Local.commit) promises2) mem2.
 Proof.
   destruct lc1. s.
-  eexists _, _. econs; memtac.
+  eexists _, _. econs.
+  - s. econs 1. admit.
   - reflexivity.
-  - admit. (* commit.wf *)
-  - econs; memtac.
-    + instantiate (1 := LT). admit. (* memory disjoint *)
-    + admit. (* wf capability *)
+  - apply WF1.
+  - apply WF1.
 Admitted.
 
 Lemma progress_silent_step
@@ -82,22 +81,19 @@ Lemma progress_read_step
       lc1 mem1
       loc ord ts
       (WF1: Local.wf lc1 mem1)
-      (PROMISE1: lc1.(Local.promise) = Memory.bot)
+      (PROMISE1: lc1.(Local.promises) = Promises.bot)
       (MAX: max_timestamp loc ts mem1):
   exists val released lc2,
     Local.read_step lc1 mem1 loc ts val released ord lc2.
 Proof.
   inv MAX. destruct msg.
-  eexists _, _, _. econs; eauto.
-  - eapply CommitFacts.read_min_spec; try apply WF1; eauto.
-    + admit. (* readable *)
-    + admit. (* readable *)
-  - (* TODO: redundant proof? *)
-    unfold CommitFacts.read_min. econs; committac; try apply WF1.
-    + unfold Capability.join_if. condtac; committac; try apply WF1.
-      inv WF1. inv MEMORY. exploit WF; eauto.
-    + inv WF1. inv MEMORY. exploit WF; eauto.
-  - rewrite PROMISE1. auto.
+  exploit (@CommitFacts.read_min_spec loc ts released); try apply WF1.
+  { admit. }
+  { admit. }
+  { inv WF1. exploit MEMORY; eauto. i. des. auto. }
+  i. des. eexists _, _, _. econs; try apply READ; eauto.
+  - rewrite PROMISE1, Promises.bot_spec. auto.
+  - admit. (* commit.closed *)
 Admitted.
 
 Lemma progress_fulfill_step
@@ -105,24 +101,25 @@ Lemma progress_fulfill_step
       loc from to val released ord
       (LT: Time.lt from to)
       (WF1: Local.wf lc1 mem1)
-      (PROMISE1: lc1.(Local.promise) = Memory.singleton loc (Message.mk val released) LT):
+      (GET1: Memory.get loc to mem1 = Some (Message.mk val released))
+      (PROMISE1: lc1.(Local.promises) = Promises.set loc to Promises.bot):
   exists lc2,
     Local.fulfill_step lc1 mem1 loc from to val released ord lc2.
 Proof.
-  exploit (@CommitFacts.write_min_spec loc to val released);
+  exploit (@CommitFacts.write_min_spec loc to released);
     try apply WF1; eauto.
   { admit. (* writable *) }
   { admit. (* writable *) }
   { admit. (* released <= m.released *) }
   { admit. (* current <= m.released for acqrel *) }
-  { inv WF1. memtac. apply Memory.join_get; memtac.
-    rewrite PROMISE1. apply Memory.singleton_get.
-  }
-  { admit. (* wf_capability m.released *) }
+  { admit. (* closed_capability m.released *) }
   i. des.
-  eexists (Local.mk _ Memory.bot). econs; eauto.
-  econs; memtac.
-  rewrite Memory.join_comm, Memory.bot_join. eauto.
+  eexists (Local.mk _ _). econs; eauto.
+  - econs; eauto.
+    rewrite PROMISE1. rewrite Promises.set_o.
+    destruct (Loc.eq_dec loc loc); [|congruence].
+    destruct (Time.eq_dec to to); [|congruence].
+    auto.
 Admitted.
 
 Lemma progress_write_step
@@ -131,21 +128,21 @@ Lemma progress_write_step
       (MAX: max_timestamp loc from mem1)
       (LT: Time.lt from to)
       (WF1: Local.wf lc1 mem1)
-      (PROMISE1: lc1.(Local.promise) = Memory.bot):
+      (PROMISE1: lc1.(Local.promises) = Promises.bot):
   exists lc2 mem2,
     Local.write_step lc1 mem1 loc from to val released ord lc2 mem2.
 Proof.
   destruct lc1. ss. subst.
   exploit progress_promise_step; eauto. s. i. des.
-  assert (promise2 = Memory.singleton loc (Message.mk val released) LT).
-  { inv x0. inv MEMORY; ss.
-    - rewrite Memory.join_comm, Memory.bot_join.
-      f_equal. apply proof_irrelevance.
-    - admit. (* invert [bot = join _ singleton] *)
-  }
-  exploit (@progress_fulfill_step (Local.mk commit promise2)); eauto.
+  assert (promises2 = Promises.set loc to Promises.bot); subst.
+  { inv x0. ss. inv PROMISE; eauto. }
+  exploit (@progress_fulfill_step (Local.mk commit (Promises.set loc to Promises.bot))); s; eauto.
   { eapply Local.promise_step_future; eauto. }
-  s. i. des.
+  { inv x0. ss. inv PROMISE.
+    - eapply Memory.add_get2. eauto.
+    - eapply Memory.split_get2. eauto.
+  }
+  i. des.
   eexists _, _. econs 2; eauto.
 Admitted.
 
@@ -153,11 +150,12 @@ Lemma progress_fence_step
       lc1 mem1
       ordr ordw
       (WF1: Local.wf lc1 mem1)
-      (PROMISE1: lc1.(Local.promise) = Memory.bot):
+      (PROMISE1: lc1.(Local.promises) = Promises.bot):
   exists lc2,
     Local.fence_step lc1 mem1 ordr ordw lc2.
 Proof.
   exploit CommitFacts.read_fence_min_spec; try apply WF1; eauto. i. des.
-  exploit CommitFacts.write_fence_min_spec; try apply WF1; eauto. i. des.
+  exploit CommitFacts.write_fence_min_spec; try apply WF; try apply WF1; eauto. i. des.
   eexists. econs; eauto.
-Qed.
+  admit. (* commit.closed *)
+Admitted.
