src/opt/ReorderCommit.v
@@ -1,0 +1,330 @@
+Require Import Basics.
+Require Import Bool.
+Require Import List.
+
+Require Import sflib.
+Require Import paco.
+Require Import respectful5.
+
+Require Import Basic.
+Require Import Event.
+Require Import Language.
+Require Import Time.
+Require Import Memory.
+Require Import Commit.
+Require Import Thread.
+
+Require Import Configuration.
+Require Import Simulation.
+Require Import Compatibility.
+Require Import MemInv.
+Require Import Progress.
+
+Require Import Syntax.
+Require Import Semantics.
+
+Set Implicit Arguments.
+
+
+Lemma read_read
+      loc1 ts1 released1 ord1
+      loc2 ts2 released2 ord2
+      commit0 commit1 commit2
+      (COMMIT1: Commit.read commit0 loc1 ts1 released1 ord1 commit1)
+      (COMMIT2: Commit.read commit1 loc2 ts2 released2 ord2 commit2)
+      (WF0: Commit.wf commit0):
+  <<COMMIT1': Commit.read commit0 loc2 ts2 released2 ord2 (CommitFacts.read_min loc2 ts2 released2 ord2 commit0)>> /\
+  <<COMMIT2': Commit.read (CommitFacts.read_min loc2 ts2 released2 ord2 commit0) loc1 ts1 released1 ord1 commit2>>.
+Proof.
+  exploit CommitFacts.read_min_spec.
+  { etrans. inv COMMIT1. apply MONOTONE. apply COMMIT2. }
+  { etrans. inv COMMIT1. apply MONOTONE. apply COMMIT2. eauto. }
+  { auto. }
+  { inv COMMIT2. apply WF_RELEASED. }
+  i.
+  exploit CommitFacts.read_min_spec.
+  { admit. }
+  { admit. }
+  { apply x0. }
+  { inv COMMIT1. apply WF_RELEASED. }
+  i.
+  splits; eauto. eapply CommitFacts.read_mon2; eauto; try apply COMMIT2.
+  inv COMMIT1. inv COMMIT2. inv MONOTONE. inv MONOTONE0.
+  econs; committac; try by etrans; eauto.
+  - rewrite RA; auto.
+  - etrans; eauto. apply WF1.
+  - etrans; eauto. apply CURRENT0.
+  - etrans; eauto. etrans.
+    + apply CURRENT0.
+    + apply WF1.
+Admitted.
+
+Lemma read_write
+      loc1 ts1 released1 ord1
+      loc2 ts2 released2 ord2
+      commit0 commit1 commit2
+      (COMMIT1: Commit.read commit0 loc1 ts1 released1 ord1 commit1)
+      (COMMIT2: Commit.write commit1 loc2 ts2 released2 ord2 commit2)
+      (LOC: loc1 <> loc2)
+      (ORD: Ordering.le Ordering.seqcst ord2 -> Ordering.le Ordering.seqcst ord1 -> False)
+      (WF0: Commit.wf commit0):
+  <<COMMIT1': Commit.write commit0 loc2 ts2 released2 ord2 (CommitFacts.write_min loc2 ts2 released2 commit0)>> /\
+  <<COMMIT2': Commit.read (CommitFacts.write_min loc2 ts2 released2 commit0) loc1 ts1 released1 ord1 commit2>>.
+Proof.
+  exploit CommitFacts.write_min_spec.
+  { inv COMMIT2. apply RELEASED. }
+  { etrans. inv COMMIT1. apply MONOTONE. apply COMMIT2. }
+  { etrans. inv COMMIT1. apply MONOTONE. apply COMMIT2. }
+  { i. splits.
+    - etrans. inv COMMIT1. apply MONOTONE. apply COMMIT2. eauto.
+    - apply COMMIT2. auto.
+  }
+  { auto. }
+  { apply COMMIT2. }
+  i.
+  exploit CommitFacts.read_min_spec.
+  { admit. }
+  { admit. }
+  { apply x0. }
+  { inv COMMIT1. apply WF_RELEASED. }
+  i.
+  splits; eauto. eapply CommitFacts.read_mon2; eauto; try apply COMMIT2.
+  inv COMMIT1. inv COMMIT2. inv MONOTONE. inv MONOTONE0.
+  econs; committac; try by etrans; eauto.
+  - rewrite RA; auto.
+  - etrans; eauto. apply WF1.
+  - etrans; eauto. etrans; apply WF1.
+  - etrans; eauto. apply CURRENT0.
+  - etrans; eauto. etrans.
+    + apply CURRENT0.
+    + apply WF1.
+  - unfold LocFun.add, LocFun.find. condtac; committac.
+    etrans; eauto.
+Admitted.
+
+Lemma read_read_fence
+      loc1 ts1 released1 ord1
+      ord2
+      commit0 commit1 commit2
+      (COMMIT1: Commit.read commit0 loc1 ts1 released1 ord1 commit1)
+      (COMMIT2: Commit.read_fence commit1 ord2 commit2)
+      (WF0: Commit.wf commit0):
+  <<COMMIT1': Commit.read_fence commit0 ord2 (CommitFacts.read_fence_min ord2 commit0)>> /\
+  <<COMMIT2': Commit.read (CommitFacts.read_fence_min ord2 commit0) loc1 ts1 released1 ord1 commit2>>.
+Proof.
+  exploit CommitFacts.read_fence_min_spec; eauto. i.
+  exploit CommitFacts.read_min_spec.
+  { admit. }
+  { admit. }
+  { apply x0. }
+  { inv COMMIT1. apply WF_RELEASED. }
+  i.
+  splits; eauto. eapply CommitFacts.read_mon2; eauto; try apply COMMIT2.
+  inv COMMIT1. inv COMMIT2. inv MONOTONE. inv MONOTONE0.
+  econs; committac; try by etrans; eauto.
+  - rewrite RA; auto.
+  - etrans; eauto. apply CURRENT0.
+  - etrans; eauto. etrans; eauto.
+    + apply CURRENT0.
+    + apply WF1.
+Admitted.
+
+Lemma read_write_fence
+      loc1 ts1 released1 ord1
+      ord2
+      commit0 commit1 commit2
+      (COMMIT1: Commit.read commit0 loc1 ts1 released1 ord1 commit1)
+      (COMMIT2: Commit.write_fence commit1 ord2 commit2)
+      (WF0: Commit.wf commit0):
+  <<COMMIT1': Commit.write_fence commit0 ord2 (CommitFacts.write_fence_min ord2 commit0)>> /\
+  <<COMMIT2': Commit.read (CommitFacts.write_fence_min ord2 commit0) loc1 ts1 released1 ord1 commit2>>.
+Proof.
+  exploit CommitFacts.write_fence_min_spec; eauto. i.
+  exploit CommitFacts.read_min_spec.
+  { admit. }
+  { admit. }
+  { apply x0. }
+  { inv COMMIT1. apply WF_RELEASED. }
+  i.
+  splits; eauto. eapply CommitFacts.read_mon2; eauto; try apply COMMIT2.
+  inv COMMIT1. inv COMMIT2. inv MONOTONE. inv MONOTONE0.
+  econs; committac; try by etrans; eauto.
+  - rewrite RA; auto.
+  - econs; s.
+    + etrans; eauto. apply CURRENT.
+    + etrans; [apply CURRENT|]. apply CURRENT0.
+    + etrans; [apply CURRENT|]. apply CURRENT0.
+  - etrans; eauto. apply CURRENT0.
+  - etrans; eauto. etrans.
+    + apply CURRENT0.
+    + apply WF1.
+Admitted.
+
+Lemma write_read
+      loc1 ts1 released1 ord1
+      loc2 ts2 released2 ord2
+      commit0 commit1 commit2
+      (COMMIT1: Commit.write commit0 loc1 ts1 released1 ord1 commit1)
+      (COMMIT2: Commit.read commit1 loc2 ts2 released2 ord2 commit2)
+      (LOC: loc1 <> loc2)
+      (ORD1: Ordering.le ord1 Ordering.relaxed)
+      (ORD2: Ordering.le ord2 Ordering.relaxed)
+      (WF0: Commit.wf commit0):
+  <<COMMIT1': Commit.read commit0 loc2 ts2 released2 ord2 (CommitFacts.read_min loc2 ts2 released2 ord2 commit0)>> /\
+  <<COMMIT2': Commit.write (CommitFacts.read_min loc2 ts2 released2 ord2 commit0) loc1 ts1 released1 ord1 commit2>>.
+Proof.
+  exploit CommitFacts.read_min_spec.
+  { inv COMMIT1. etrans. apply MONOTONE. apply COMMIT2. }
+  { inv COMMIT1. etrans. apply MONOTONE. apply COMMIT2. eauto. }
+  { apply WF0. }
+  { inv COMMIT2. apply WF_RELEASED. }
+  i.
+  exploit CommitFacts.write_min_spec.
+  { admit. }
+  { admit. }
+  { admit. }
+  { admit. }
+  { apply x0. }
+  { inv COMMIT1. apply WF_RELEASED. }
+  i.
+  splits; eauto. eapply CommitFacts.write_mon2; eauto; try apply COMMIT2.
+  inv COMMIT1. inv COMMIT2. inv MONOTONE. inv MONOTONE0.
+  econs; committac; try by etrans; eauto.
+  - rewrite RW3. apply WF1.
+  - etrans; eauto. apply CURRENT0.
+  - etrans; eauto. etrans.
+    + apply CURRENT0.
+    + apply WF1.
+  - etrans; eauto. etrans.
+    + apply CURRENT0.
+    + etrans; apply WF1.
+  - unfold LocFun.add, LocFun.find. condtac; committac.
+    + etrans; eauto.
+    + etrans; eauto.
+Admitted.
+
+Lemma write_write
+      loc1 ts1 released1 ord1
+      loc2 ts2 released2 ord2
+      commit0 commit1 commit2
+      (COMMIT1: Commit.write commit0 loc1 ts1 released1 ord1 commit1)
+      (COMMIT2: Commit.write commit1 loc2 ts2 released2 ord2 commit2)
+      (LOC: loc1 <> loc2)
+      (ORD1: Ordering.le ord1 Ordering.relaxed)
+      (WF0: Commit.wf commit0):
+  <<COMMIT1': Commit.write commit0 loc2 ts2 released2 ord2 (CommitFacts.write_min loc2 ts2 released2 commit0)>> /\
+  <<COMMIT2': Commit.write (CommitFacts.write_min loc2 ts2 released2 commit0) loc1 ts1 released1 ord1 commit2>>.
+Proof.
+  exploit CommitFacts.write_min_spec.
+  { inv COMMIT2. apply RELEASED. }
+  { etrans. inv COMMIT1. apply MONOTONE. apply COMMIT2. }
+  { etrans. inv COMMIT1. apply MONOTONE. apply COMMIT2. }
+  { i. splits.
+    - etrans. inv COMMIT1. apply MONOTONE. apply COMMIT2. eauto.
+    - apply COMMIT2. auto.
+  }
+  { auto. }
+  { apply COMMIT2. }
+  i.
+  exploit CommitFacts.write_min_spec.
+  { admit. }
+  { admit. }
+  { admit. }
+  { admit. }
+  { apply x0. }
+  { inv COMMIT1. apply WF_RELEASED. }
+  i.
+  splits; eauto. eapply CommitFacts.write_mon2; eauto; try apply COMMIT2.
+  inv COMMIT1. inv COMMIT2. inv MONOTONE. inv MONOTONE0.
+  econs; committac; try by etrans; eauto.
+  - rewrite RW3. apply WF1.
+  - etrans; eauto. etrans; apply WF1.
+  - etrans; eauto. apply CURRENT0.
+  - etrans; eauto. etrans.
+    + apply CURRENT0.
+    + apply WF1.
+  - etrans; eauto. etrans.
+    + apply CURRENT0.
+    + etrans; apply WF1.
+  - unfold LocFun.add, LocFun.find. repeat condtac; committac.
+    + etrans; eauto.
+    + etrans; eauto.
+Admitted.
+
+Lemma read_fence_write
+      ord1
+      loc2 ts2 released2 ord2
+      commit0 commit1 commit2
+      (COMMIT1: Commit.read_fence commit0 ord1 commit1)
+      (COMMIT2: Commit.write commit1 loc2 ts2 released2 ord2 commit2)
+      (ORD1: Ordering.le ord1 Ordering.acqrel)
+      (WF0: Commit.wf commit0):
+  <<COMMIT1': Commit.write commit0 loc2 ts2 released2 ord2 (CommitFacts.write_min loc2 ts2 released2 commit0)>> /\
+  <<COMMIT2': Commit.read_fence (CommitFacts.write_min loc2 ts2 released2 commit0) ord1 commit2>>.
+Proof.
+  exploit CommitFacts.write_min_spec.
+  { inv COMMIT2. apply RELEASED. }
+  { etrans. inv COMMIT1. apply MONOTONE. apply COMMIT2. }
+  { etrans. inv COMMIT1. apply MONOTONE. apply COMMIT2. }
+  { i. splits.
+    - etrans. inv COMMIT1. apply MONOTONE. apply COMMIT2. eauto.
+    - apply COMMIT2. auto.
+  }
+  { auto. }
+  { apply COMMIT2. }
+  i.
+  exploit CommitFacts.read_fence_min_spec.
+  { apply x0. }
+  i.
+  splits; eauto. eapply CommitFacts.read_fence_mon2; eauto; try apply COMMIT2.
+  inv COMMIT1. inv COMMIT2. inv MONOTONE. inv MONOTONE0.
+  econs; committac; try by etrans; eauto.
+  - rewrite RA; auto.
+  - etrans; eauto. apply WF1.
+  - etrans; eauto. etrans; apply WF1.
+  - unfold LocFun.add, LocFun.find. condtac; committac.
+    etrans; eauto.
+Qed.
+
+Lemma write_fence_write
+      ord1
+      loc2 ts2 released2 ord2
+      commit0 commit1 commit2
+      (COMMIT1: Commit.write_fence commit0 ord1 commit1)
+      (COMMIT2: Commit.write commit1 loc2 ts2 released2 ord2 commit2)
+      (ORD1: Ordering.le ord1 Ordering.relaxed)
+      (WF0: Commit.wf commit0):
+  <<COMMIT1': Commit.write commit0 loc2 ts2 released2 ord2 (CommitFacts.write_min loc2 ts2 released2 commit0)>> /\
+  <<COMMIT2': Commit.write_fence (CommitFacts.write_min loc2 ts2 released2 commit0) ord1 commit2>>.
+Proof.
+  exploit CommitFacts.write_min_spec.
+  { inv COMMIT2. apply RELEASED. }
+  { etrans. inv COMMIT1. apply MONOTONE. apply COMMIT2. }
+  { etrans. inv COMMIT1. apply MONOTONE. apply COMMIT2. }
+  { i. splits.
+    - etrans. inv COMMIT1. apply MONOTONE. apply COMMIT2. eauto.
+    - apply COMMIT2. auto.
+  }
+  { auto. }
+  { apply COMMIT2. }
+  i.
+  exploit CommitFacts.write_fence_min_spec.
+  { apply x0. }
+  i.
+  splits; eauto. eapply CommitFacts.write_fence_mon2; eauto; try apply COMMIT2.
+  inv COMMIT1. inv COMMIT2. inv MONOTONE. inv MONOTONE0.
+  econs; committac; try by etrans; eauto.
+  - econs; s; committac.
+    + rewrite RLX; auto. apply CURRENT0.
+    + etrans; eauto. etrans.
+      * apply CURRENT0.
+      * apply WF1.
+    + etrans; eauto. apply WF1.
+    + etrans; eauto. apply CURRENT. apply CURRENT0.
+    + etrans; eauto. etrans; apply WF1.
+  - rewrite RW2. apply WF1.
+  - rewrite RW2. etrans; apply WF1.
+  - unfold LocFun.add, LocFun.find.
+    committac; try by destruct ord1; inv ORD1; inv H.
+    condtac; committac. etrans; eauto.
+Qed.
