src/opt/ReorderStep.v
@@ -19,7 +19,9 @@ Require Import Simulation.
 Require Import Compatibility.
 Require Import MemInv.
 Require Import Progress.
-Require Import ReorderMemory.
+
+Require ReorderMemory.
+Require ReorderCommit.
 
 Require Import Syntax.
 Require Import Semantics.
@@ -30,7 +32,7 @@ Set Implicit Arguments.
 Lemma progress_step
       rs1 i1 s1 lc1 mem1
       (WF1: Local.wf lc1 mem1)
-      (PROMISE1: lc1.(Local.promise) = Memory.bot):
+      (PROMISES1: lc1.(Local.promises) = Promises.bot):
   (exists lc2, <<STEP: Thread.internal_step (Thread.mk lang (State.mk rs1 (i1::s1)) lc1 mem1) lc2>>) \/
   (exists e lc2, <<STEP: Thread.external_step e (Thread.mk lang (State.mk rs1 (i1::s1)) lc1 mem1) lc2>>).
 Proof.
@@ -93,47 +95,15 @@ Lemma reorder_read_read
     <<STEP2: Local.read_step lc1' mem0 loc1 ts1 val1 released1 ord1 lc2>>.
 Proof.
   inv STEP1. inv STEP2. ss.
-  exploit CommitFacts.read_min_spec; try apply WF0; try apply GET0; eauto.
-  { eapply Capability.readable_mon; try apply COMMIT0; eauto. apply COMMIT. }
-  i. des.
-  exploit CommitFacts.read_min_spec; try apply WF; try apply GET; eauto.
-  { eapply Capability.le_on_readable; eauto. apply COMMIT. }
+  exploit ReorderCommit.read_read; try apply COMMIT; try apply COMMIT0; eauto.
   { apply WF0. }
   i. des.
   eexists. splits.
   - econs; eauto.
-  - destruct lc0. s. econs; try eapply CommitFacts.read_mon2; eauto.
-    s. inv COMMIT. inv COMMIT0. inv MONOTONE. inv MONOTONE0.
-    unfold CommitFacts.read_min.
-    destruct (Ordering.le_dec Ordering.acqrel ord2).
-    { rewrite ORD2 in l. inv l. }
-    econs; committac.
-    + condtac; committac.
-      * rewrite ACQUIRE; auto.
-      * rewrite CURRENT1. auto.
-      * rewrite CURRENT1. auto.
-      * rewrite READ1. apply CURRENT2.
-    + rewrite CURRENT1. auto.
-    + rewrite CURRENT1. auto.
-    + rewrite READ1. apply CURRENT2.
-    + rewrite RELEASED. auto.
-    + rewrite ACQUIRABLE. auto.
-    + rewrite ACQUIRABLE1. auto.
-Qed.
-
-Lemma reorder_memory_get_promise
-      promise0 mem0 loc from to msg promise1 mem1
-      l t m
-      (LE: Memory.le promise0 mem0)
-      (GET1: Memory.get l t mem0 = Some m)
-      (GET2: Memory.get l t promise0 = None)
-      (PROMISE: Memory.promise promise0 mem0 loc from to msg promise1 mem1):
-  Memory.get l t mem1 = Some m /\
-  Memory.get l t promise1 = None.
-Proof.
-  exploit reorder_memory_get_promise_iff; eauto. intros [X1 X2].
-  apply X1. auto.
-Qed.
+    + apply COMMIT1'.
+    + admit.
+  - refine (Local.step_read _ _ _ _ _ _); eauto.
+Admitted.
 
 Lemma reorder_read_promise
       loc1 ts1 val1 released1 ord1
@@ -149,15 +119,12 @@ Lemma reorder_read_promise
     <<STEP2: Local.read_step lc1' mem2 loc1 ts1 val1 released1 ord1 lc2>>.
 Proof.
   inv STEP1. inv STEP2. ss.
-  exploit reorder_memory_get_promise; try apply WF0; eauto. i. des.
+  exploit ReorderMemory.get_promise_inv; try apply WF0; eauto. i. des.
   exploit Memory.promise_future; try apply WF0; eauto. i. des.
-  exploit Commit.future_wf; try apply WF0; eauto. i.
-  exploit Memory.future_get; eauto. i.
-  exploit CommitFacts.read_min_spec; try apply COMMIT; eauto. i. des.
+  exploit Commit.future_closed; try apply WF0; eauto. i.
   eexists. splits.
-  - econs; try reflexivity; try apply MEMORY; eauto.
-  - destruct lc0. ss. econs; try eapply CommitFacts.read_mon2; eauto.
-    rewrite <- COMMIT0. apply CommitFacts.read_min_min. auto.
+  - econs; try apply WF0; eauto. reflexivity.
+  - econs; eauto. s. eapply CommitFacts.read_mon2; eauto.
 Qed.
 
 Lemma reorder_read_fulfill
@@ -176,38 +143,17 @@ Lemma reorder_read_fulfill
     <<STEP2: Local.read_step lc1' mem0 loc1 ts1 val1 released1 ord1 lc2>>.
 Proof.
   inv STEP1. inv STEP2. ss.
-  exploit Memory.fulfill_get; eauto. i.
-  exploit Memory.le_get; try apply WF0; eauto. i.
-  exploit CommitFacts.write_min_spec; try apply x1; try apply WF0; eauto.
-  { eapply Capability.writable_mon; try apply COMMIT0; eauto. apply COMMIT. }
-  { etrans; [apply COMMIT|]. apply COMMIT0. }
-  { instantiate (1 := ord2). i. inv COMMIT0.
-    rewrite <- RELEASED0; auto. apply Capability.incr_writes_mon. apply COMMIT.
-  }
-  { inv WF0. inv MEMORY0. exploit WF; eauto. }
-  i. des.
-  exploit CommitFacts.read_min_spec; try apply GET; eauto.
-  { eapply Capability.le_on_readable; eauto. apply COMMIT. }
+  exploit ReorderCommit.read_write; try apply COMMIT; try apply COMMIT0; eauto.
   { apply WF0. }
   i. des.
   eexists. splits.
   - econs; eauto.
-  - destruct lc0. ss. econs; try eapply CommitFacts.read_mon2; eauto.
-    + inv COMMIT. inv COMMIT0. inv MONOTONE. inv MONOTONE0.
-      unfold CommitFacts.read_min, CommitFacts.write_min. ss.
-      econs; committac; try condtac; committac.
-      * rewrite ACQUIRE; auto.
-      * rewrite CURRENT1. auto.
-      * rewrite READ0. apply CURRENT2.
-      * rewrite CURRENT1. auto.
-      * rewrite READ0. apply CURRENT2.
-      * unfold LocFun.add, LocFun.find.
-        condtac; committac.
-        etrans; [apply RELEASED|apply RELEASED4].
-      * rewrite ACQUIRABLE. auto.
-      * rewrite ACQUIRABLE0. auto.
-    + erewrite <- reorder_memory_get_fulfill; eauto. apply WF0.
-Qed.
+    + apply COMMIT1'.
+    + admit.
+  - refine (Local.step_read _ _ _ _ _ _); eauto.
+    s. inv FULFILL. rewrite Promises.unset_o.
+    condtac; auto.
+Admitted.
 
 Lemma reorder_read_write
       loc1 ts1 val1 released1 ord1
@@ -245,6 +191,7 @@ Lemma reorder_read_fence
       (ORD1: Ordering.le Ordering.relaxed ord1)
       (ORDR2: Ordering.le ordr2 Ordering.relaxed)
       (ORDW2: Ordering.le ordw2 Ordering.acqrel)
+      (RLX: Ordering.le Ordering.relaxed ordw2 -> Ordering.le ord1 Ordering.relaxed)
       (WF0: Local.wf lc0 mem0)
       (STEP1: Local.read_step lc0 mem0 loc1 ts1 val1 released1 ord1 lc1)
       (STEP2: Local.fence_step lc1 mem0 ordr2 ordw2 lc2):
@@ -253,53 +200,18 @@ Lemma reorder_read_fence
     <<STEP2: Local.read_step lc1' mem0 loc1 ts1 val1 released1 ord1 lc2>>.
 Proof.
   inv STEP1. inv STEP2. ss.
-  destruct (Ordering.le_dec Ordering.acqrel ordr2) eqn:ORDR2'; committac.
-  { clear ORDR2'. rewrite ORDR2 in l. inv l. }
-  destruct (Ordering.le_dec Ordering.relaxed ord1) eqn:ORD1'; committac.
-  exploit CommitFacts.fence_min_spec; try apply WF0; eauto. i. des.
-  exploit CommitFacts.read_min_spec; try apply WF; try apply GET; eauto.
-  { unfold CommitFacts.fence_min. rewrite ORDR2'.
-    instantiate (2 := ordw2). committac.
-    inv COMMIT. inv READABLE. econs; ss.
-    - i. unfold TimeMap.get, LocFun.find. committac; eauto.
-      condtac; committac; eauto.
-    - unfold TimeMap.get, LocFun.find. committac; eauto.
-      condtac; committac. eauto.
-  }
+  exploit ReorderCommit.read_read_fence; try apply COMMIT; try apply READ; eauto.
   { apply WF0. }
+  i. des.
+  exploit ReorderCommit.read_write_fence; try apply COMMIT2'; try apply WRITE; eauto.
+  { apply COMMIT1'. }
   i. des.
   eexists. splits.
   - econs; eauto.
-  - destruct lc0. s. econs; try eapply CommitFacts.read_mon2; eauto.
-    inv COMMIT. inv COMMIT0. inv MONOTONE. inv MONOTONE0.
-    unfold CommitFacts.read_min, CommitFacts.fence_min.
-    rewrite ORDR2'. committac.
-    econs; committac; try condtac; committac.
-    + rewrite ACQUIRE; auto.
-    + rewrite CURRENT0. auto.
-    + condtac; committac.
-      * econs; committac.
-        { etrans; [apply CURRENT0|apply CURRENT1]. }
-        { etrans; [apply CURRENT0|apply RELAXED; auto]. }
-      * rewrite CURRENT0. auto.
-    + rewrite CURRENT0. auto.
-    + rewrite READ0. apply CURRENT1.
-    + rewrite CURRENT0. auto.
-    + econs; committac.
-      * etrans; [apply CURRENT0|apply CURRENT1].
-      * etrans; [apply CURRENT0|apply RELAXED; auto].
-    + rewrite CURRENT0. auto.
-    + rewrite CURRENT0. auto.
-    + rewrite READ0. apply CURRENT1.
-    + unfold LocFun.find. committac.
-      * rewrite CURRENT0. eauto.
-      * etrans; [apply RELEASED|apply RELEASED0].
-    + unfold LocFun.find. committac.
-      * etrans; [apply RELEASED|apply RELEASED0].
-      * etrans; [apply RELEASED|apply RELEASED0].
-    + rewrite ACQUIRABLE. auto.
-    + rewrite ACQUIRABLE0. auto.
-Qed.
+    + apply COMMIT1'0.
+    + admit.
+  - refine (Local.step_read _ _ _ _ _ _); eauto.
+Admitted.
 
 Lemma reorder_fulfill_read
       loc1 from1 to1 val1 released1 ord1
@@ -318,35 +230,19 @@ Lemma reorder_fulfill_read
     <<STEP2: Local.fulfill_step lc1' mem0 loc1 from1 to1 val1 released1 ord1 lc2>>.
 Proof.
   inv STEP1. inv STEP2. ss.
-  exploit Memory.fulfill_get; eauto. i.
-  exploit Memory.le_get; try apply WF0; eauto. i.
-  exploit CommitFacts.read_min_spec; try apply WF0; try apply GET; eauto.
-  { eapply Capability.readable_mon; try apply COMMIT0; eauto. apply COMMIT. }
-  i. des.
-  exploit CommitFacts.write_min_spec; try apply x1; eauto.
-  { eapply Capability.le_on_writable; eauto. apply COMMIT. }
-  { s. apply COMMIT. }
-  { instantiate (1 := ord1). i. rewrite ORD1 in H. inv H. }
+  exploit ReorderCommit.write_read; try apply COMMIT; try apply COMMIT0; eauto.
   { apply WF0. }
-  { inv WF0. inv MEMORY0. exploit WF0; eauto. }
   i. des.
   eexists. splits.
-  - econs; eauto. erewrite reorder_memory_get_fulfill; eauto. apply WF0.
-  - destruct lc0. s. econs; try eapply CommitFacts.write_mon2; eauto.
-    inv COMMIT. inv COMMIT0. inv MONOTONE. inv MONOTONE0.
-    unfold CommitFacts.write_min, CommitFacts.read_min.
-    condtac; committac.
-    { rewrite ORD2 in l. inv l. }
-    econs; committac.
-    + rewrite CURRENT1. auto.
-    + rewrite CURRENT1. auto.
-    + rewrite WRITE0. apply CURRENT2.
-    + unfold LocFun.add, LocFun.find.
-      condtac; committac.
-      * rewrite RELEASED3. apply RELEASED4.
-      * etrans; [apply RELEASED|apply RELEASED4].
-    + rewrite ACQUIRABLE0. auto.
-Qed.
+  - econs; eauto.
+    + contradict PROMISES.
+      inv FULFILL. rewrite Promises.unset_o.
+      condtac; auto.
+      destruct (Loc.eq_dec loc2 loc1); [congruence|]. auto.
+    + apply COMMIT1'.
+    + admit.
+  - econs; eauto.
+Admitted.
 
 Lemma reorder_fulfill_promise
       loc1 from1 to1 val1 released1 ord1
@@ -362,18 +258,12 @@ Lemma reorder_fulfill_promise
     <<STEP2: Local.fulfill_step lc1' mem2 loc1 from1 to1 val1 released1 ord1 lc2>>.
 Proof.
   inv STEP1. inv STEP2. ss.
-  exploit reorder_memory_fulfill_promise; try apply MEMORY; try apply WF0; eauto. i. des.
+  exploit ReorderMemory.fulfill_promise; try apply MEMORY; try apply WF0; eauto. i. des.
   exploit Memory.promise_future; try apply x0; try apply WF0; eauto. i. des.
-  exploit Commit.future_wf; try apply WF0; eauto. i.
-  exploit Memory.fulfill_get; try apply x0; eauto. i.
-  exploit Memory.le_get; try apply LE2; eauto. i.
-  exploit CommitFacts.write_min_spec; try apply COMMIT; eauto.
-  { inv WF2. exploit WF; eauto. }
-  i. des.
+  exploit Commit.future_closed; try apply WF0; eauto. i.
   eexists. splits.
-  - econs; try reflexivity; try apply x0; eauto.
-  - destruct lc0. ss. econs; try eapply CommitFacts.write_mon2; eauto.
-    rewrite <- COMMIT0. eapply CommitFacts.write_min_min. eauto.
+  - econs; try apply WF0; eauto. reflexivity.
+  - econs; eauto. s. eapply CommitFacts.write_mon2; eauto.
 Qed.
 
 Lemma reorder_fulfill_fulfill
@@ -392,46 +282,16 @@ Lemma reorder_fulfill_fulfill
     <<STEP2: Local.fulfill_step lc1' mem0 loc1 from1 to1 val1 released1 ord1 lc2>>.
 Proof.
   inv STEP1. inv STEP2. ss.
-  exploit reorder_memory_fulfill_fulfill; try apply MEMORY; eauto. i. des.
-  exploit Memory.fulfill_get; try apply x0; eauto. i.
-  exploit Memory.le_get; try apply WF0; eauto. i.
-  exploit CommitFacts.write_min_spec; try apply x3; try apply WF0; eauto.
-  { eapply Capability.writable_mon; try apply COMMIT0; eauto. apply COMMIT. }
-  { etrans; [apply COMMIT|]. apply COMMIT0. }
-  { instantiate (1 := ord2). committac.
-    - inv COMMIT0. rewrite <- RELEASED0; auto.
-      etrans; [apply COMMIT|]. committac.
-    - inv COMMIT0. etrans; [|apply RELEASED0; auto].
-      s. apply TimeMap.incr_ts.
-  }
-  { inv WF0. inv MEMORY1. exploit WF; eauto. }
-  i. des.
-  exploit Memory.fulfill_get; try apply x1; eauto. i.
-  exploit Memory.le_get; try apply x4; eauto.
-  { eapply Memory.fulfill_future; eauto. apply WF0. }
-  i.
-  exploit CommitFacts.write_min_spec; try apply x5; eauto.
-  { eapply Capability.le_on_writable; eauto. apply COMMIT. }
-  { committac. unfold LocFun.add, LocFun.find.
-    condtac; [congruence|]. apply COMMIT.
-  }
-  { instantiate (1 := ord1). i. rewrite ORD1 in H. inv H. }
+  exploit ReorderMemory.fulfill_fulfill; try apply FULFILL; try apply FULFILL0. i. des.
+  exploit ReorderCommit.write_write; try apply COMMIT; try apply COMMIT0; eauto.
   { apply WF0. }
-  { inv WF0. inv MEMORY1. exploit WF0; eauto. }
   i. des.
   eexists. splits.
   - econs; eauto.
-  - destruct lc0. ss. econs; try eapply CommitFacts.write_mon2; eauto.
-    inv COMMIT. inv COMMIT0. inv MONOTONE. inv MONOTONE0. ss.
-    econs; committac.
-    + rewrite CURRENT1. auto.
-    + rewrite WRITE1. apply CURRENT2.
-    + unfold LocFun.add, LocFun.find.
-      repeat condtac; committac.
-      { rewrite RELEASED4. eauto. }
-      { etrans; [apply RELEASED|apply RELEASED8]. }
-    + rewrite ACQUIRABLE. auto.
-Qed.
+    + apply COMMIT1'.
+    + admit.
+  - econs; eauto.
+Admitted.
 
 Lemma reorder_fulfill_write
       loc1 from1 to1 val1 released1 ord1
@@ -451,13 +311,13 @@ Proof.
   inv STEP2.
   - exploit reorder_fulfill_fulfill; eauto. i. des.
     eexists. splits; eauto. econs 1. eauto.
-    inv STEP1. erewrite reorder_memory_cell_fulfill; eauto.
+    inv STEP1. erewrite ReorderMemory.cell_fulfill; eauto.
   - exploit reorder_fulfill_promise; eauto. i. des.
     exploit reorder_fulfill_fulfill; try apply STEP2; eauto.
     { eapply Local.promise_step_future; eauto. }
     i. des.
     eexists. splits; eauto. econs 2; eauto.
-    inv STEP1. erewrite reorder_memory_cell_fulfill; eauto.
+    inv STEP1. erewrite ReorderMemory.cell_fulfill; eauto.
 Qed.
 
 Lemma reorder_fence_promise
@@ -477,13 +337,12 @@ Lemma reorder_fence_promise
 Proof.
   inv STEP1. inv STEP2. ss.
   exploit Memory.promise_future; try apply WF0; eauto. i. des.
-  exploit Commit.future_wf; try apply WF0; eauto. i.
-  exploit CommitFacts.fence_min_spec; try apply COMMIT; eauto. i. des.
+  exploit Commit.future_closed; try apply WF0; eauto. i.
   eexists. splits.
-  - econs; try reflexivity; try apply MEMORY; eauto.
-  - destruct lc0. ss. econs; try eapply CommitFacts.fence_mon2; eauto.
-    + rewrite <- COMMIT0. apply CommitFacts.fence_min_min. auto.
-    + i. rewrite ORDW1 in H. inv H.
+  - econs; try apply WF0; eauto. reflexivity.
+  - econs; eauto.
+    + eapply CommitFacts.write_fence_mon2; eauto.
+    + i. destruct ordw1; inv ORDW1; inv H.
 Qed.
 
 Lemma reorder_fence_fulfill
@@ -501,45 +360,19 @@ Lemma reorder_fence_fulfill
     <<STEP1: Local.fulfill_step lc0 mem0 loc2 from2 to2 val2 released2 ord2 lc1'>> /\
     <<STEP2: Local.fence_step lc1' mem0 ordr1 ordw1 lc2>>.
 Proof.
-  destruct (Ordering.le_dec Ordering.acqrel ordw1) eqn:ORDW1'.
-  { clear ORDW1'. rewrite ORDW1 in l. inv l. }
   inv STEP1. inv STEP2. ss.
-  exploit Memory.fulfill_get; eauto. i.
-  exploit Memory.le_get; try apply WF0; eauto. i.
-  exploit CommitFacts.write_min_spec; try apply x1; try apply WF0; eauto.
-  { eapply Capability.writable_mon; try apply COMMIT0; eauto. apply COMMIT. }
-  { etrans; [apply COMMIT|]. apply COMMIT0. }
-  { instantiate (1 := ord2). i. inv COMMIT0.
-    rewrite <- RELEASED0; auto. apply Capability.incr_writes_mon. apply COMMIT.
-  }
-  { inv WF0. inv MEMORY0. exploit WF; eauto. }
+  exploit ReorderCommit.write_fence_write; try apply WRITE; try apply COMMIT; eauto.
+  { apply READ. }
   i. des.
-  exploit CommitFacts.fence_min_spec; eauto.
+  exploit ReorderCommit.read_fence_write; try apply READ; try apply COMMIT1'; eauto.
   { apply WF0. }
   i. des.
   eexists. splits.
   - econs; eauto.
-  - destruct lc0. ss. econs; try eapply CommitFacts.fence_mon2; eauto.
-    + inv COMMIT. inv COMMIT0. inv MONOTONE. inv MONOTONE0.
-      unfold CommitFacts.fence_min, CommitFacts.write_min.
-      committac. econs; committac.
-      * condtac; committac.
-        { rewrite ACQUIRE; auto. }
-        { rewrite CURRENT0. auto. }
-      * condtac; committac.
-        { econs; committac.
-          - etrans; [apply CURRENT0|apply CURRENT1].
-          - etrans; [apply RELAXED; auto|apply CURRENT1].
-        }
-        { rewrite CURRENT0. auto. }
-      * rewrite CURRENT0. auto.
-      * unfold LocFun.add, LocFun.find.
-        repeat condtac; committac.
-        { etrans; [apply RELEASED|apply RELEASED4]. }
-        { etrans; [apply RELEASED|apply RELEASED4]. }
-      * rewrite ACQUIRABLE. auto.
-    + i. rewrite ORDW1 in H. inv H.
-Qed.
+    + apply COMMIT1'0.
+    + admit.
+  - econs; eauto. i. destruct ordw1; inv ORDW1; inv H.
+Admitted.
 
 Lemma reorder_fence_write
       ordr1 ordw1
